wip

Examples/temp_cfi.v
@@ -4,17 +4,14 @@ Require Import -(notations) arm7_cfi2.
 Require Import Picinae_armv7.
 Require Import Lia ZifyN ZifyNat.
 Import ARM7Notations.
-Import ListNotations.
 Require Import Nat.
 
-Open Scope N.
+Open Scope Z.
 
-Definition to_a := Z.mul 4.
-Definition i2a' i2i' (i: Z) := to_a (i2i' i).
 Definition compute_table_size sr := Z.to_nat (2 ^ (32 - sr)).
 Definition compute_table_start_index tbi ti := Z.to_nat (ti - tbi).
 Definition SafeEntry i2i' (pol: Z -> list Z) ai si a :=
-  to_a ai = a \/ exists di (D: i2a' i2i' di = a), In di (pol si).
+  ai * 4 = a \/ exists di (D: (i2i' di) * 4 = a), In di (pol si).
 Definition InBlock i ilen da' :=
   (i * 4 <= Z.of_N da' < (i + Z.of_nat ilen) * 4 /\ N.divide 4 da')%Z.
 Definition SafeDest i2i' pol ai si ilen a :=
@@ -27,10 +24,11 @@ Definition extract_table sr tbi ti (flattened_tables: list Z) :=
   let table := firstn ts (skipn si flattened_tables) in
   if (si + ts <=? length flattened_tables)%nat && (tbi <=? ti)%Z then Some table else None.
 
-Definition ContainsBlock (p: program) b s i :=
+Open Scope N.
+Definition ContainsBlock b s i :=
   forall i', InBlock i (length b) (i'*4) ->
     match nth_error b (Z.to_nat (Z.of_N i' - i)) with
-    | Some z => p s (i'*4) = Some (4, arm2il (i'*4) (arm_decode z))
+    | Some z => arm_prog s (i'*4) = Some (4, arm2il (i'*4) (arm_decode z))
     | None => False
     end.
 Definition InBlockX i ilen (x: exit * store) :=
@@ -50,15 +48,68 @@ Proof.
     destruct H as [[[? ?] [? ?]] ?]. repeat split; [destruct (N.eq_dec x i); [now subst | lia] | lia | now exists x].
     easy.
 Qed.
-Lemma inblockx_cons:
-  forall i (b:Z) b' x,
-    InBlockX (i + 1) (length b') x -> InBlockX i (length (b :: b')) x.
+Lemma inblockx_ss:
+  forall i len x,
+    InBlockX (i + 1) (len) x -> InBlockX i (len+1) x.
 Proof.
   intros. destruct x, e.
     unfold InBlockX, InBlock in *. simpl in *. split. lia. easy.
     easy.
 Qed.
 
+Lemma make_jump_table_map_safety:
+  forall ai dis i2i' sl sr x,
+  In (make_jump_table_map dis (map i2i' dis) sl sr (fun _ => Z.mul ai 4) x) (Z.mul ai 4::map (fun i => Z.mul (i2i' i) 4) dis).
+Proof.
+  intros. induction dis.
+    now left.
+    cbn [make_jump_table_map map]. destruct orb.
+      right. left. now rewrite Z.mul_comm.
+      inversion IHdis.
+        now left.
+        right. now right.
+Qed.
+Lemma safeentry_in:
+  forall ai pol i2i' i x,
+    In x (Z.mul ai 4::map (fun i => Z.mul (i2i' i) 4) (pol i)) ->
+    SafeEntry i2i' pol ai i x.
+Proof.
+  intros. inversion H.
+    now left.
+    right. apply in_map_iff in H0. inversion H0. now exists x0.
+Qed.
+Lemma Forall_map2list:
+  forall P m n (H: forall a, P (m a)),
+    Forall P (_map2list m n).
+Proof.
+  intros. induction n. constructor. simpl. now constructor.
+Qed.
+Lemma SafeTable_rewrite_w_table:
+  forall irm tc pol i2i' cond i ti ai z' table tc'
+    (RWT: rewrite_w_table irm tc (pol i) i2i' cond i ti ai = Some (z', table, tc')),
+    SafeTable i2i' pol ai i table.
+Proof.
+  intros. unfold rewrite_w_table in RWT. destruct_match_in RWT; try discriminate.
+    inversion RWT; subst. apply Forall_nil.
+    remember (Z.shiftl _ _). inversion RWT. apply Forall_rev. rewrite map2list_fix. apply Forall_map2list.
+      intro. rewrite Z.mul_comm. apply safeentry_in, make_jump_table_map_safety.
+Qed.
+Lemma SafeTable_rewrite_inst:
+  forall tc i2i' z pol i ti ai bi txt z' table tc'
+    (RI: rewrite_inst tc i2i' z (pol i) i ti ai bi txt = Some (z', table, tc')),
+    SafeTable i2i' pol ai i table.
+Proof.
+  assert (forall i' ai tc a b c, goto_abort i' ai tc = Some (a, b, c) -> b = nil).
+    unfold goto_abort. intros. destruct_match_in H; now inversion H.
+  assert (forall x tc a b c, wo_table x tc = Some (a, b, c) -> b = nil).
+    unfold wo_table. intros. destruct x in H0; now inversion H0.
+  assert (forall l cond imm24 i dis i2i' ai tc a b c, rewrite_b_bl l cond imm24 i dis i2i' ai tc = Some (a, b, c) -> b = nil).
+    unfold rewrite_b_bl. intros. destruct_match_in H1; now inversion H1.
+
+  intros. unfold rewrite_inst in RI. destruct_match_in RI;
+    try solve [first [apply H in RI|apply H0 in RI|apply H1 in RI|inversion RI]; subst; constructor];
+    now apply SafeTable_rewrite_w_table in RI.
+Qed.
 
 (* copied straight from the Z proof, since there is no N version for some reason *)
 Lemma Ndivdec a b : {(a | b)} + {~ (a | b)}.
@@ -71,54 +122,45 @@ Proof.
    + left. now apply N.Lcm0.mod_divide.
    + right. now rewrite <- N.Lcm0.mod_divide.
 Defined.
-Lemma inblockx_dec : forall i ilen a, {InBlockX i ilen a} + {~InBlockX i ilen a}.
+Lemma inblock_dec : forall i ilen a, {InBlock i ilen a} + {~InBlock i ilen a}.
 Proof.
-  intros. destruct a, e.
-  unfold InBlockX, InBlock. simpl.
-  destruct (Ndivdec 4 a), (Z_le_dec (Z.of_N i * 4) (Z.of_N a)), (Z_lt_dec (Z.of_N a) (((Z.of_N i) + Z.of_nat ilen) * 4)).
+  intros. unfold InBlock.
+  destruct (Ndivdec 4 a), (Z_le_dec (i * 4) (Z.of_N a)), (Z_lt_dec (Z.of_N a) ((i + Z.of_nat ilen) * 4)).
   all: (now left) || (now right).
 Qed.
+Lemma inblockx_dec : forall i ilen a, {InBlockX i ilen a} + {~InBlockX i ilen a}.
+Proof.
+  intros. destruct a, e. apply inblock_dec. now right.
+Qed.
 
-(* for prog p that contains block b, after starting at entry index ei with store s,
-   prop P holds for all states constrained to the block as well as the first step outside the block *)
-Definition AfterBlock (P: exit * store -> Prop) b p s bi ei :=
+Definition AfterBlock (P: exit * store -> Prop) s bi len ei T :=
   forall t0 t1 a' s'
-    (XP: exec_prog p ((Addr a', s')::t1++t0))
-    (SO: ostartof t1 = Some (Addr (ei*4), s))
-    (CB: ContainsBlock p b s (Z.of_N bi))
-    (IB: Forall (InBlockX bi (length b)) t1),
+    (XP: exec_prog arm_prog ((Addr a', s')::t1++(Addr (ei*4), s)::t0))
+    (T1: Forall T t1)
+    (IB: Forall (InBlockX bi len) (t1++(Addr (ei*4), s)::nil)),
     P (Addr a', s').
 
-(* like AfterBlock, but ignores the first step outside the block *)
-Definition DuringBlock P b p s bi ei := AfterBlock (fun xs => P xs \/ ~InBlockX bi (length b) xs) b p s bi ei.
-(* an alternative definition that we prove is equivalent *)
-Definition DuringBlock' (P: _ -> Prop) b p s bi ei :=
+Definition DuringBlock P s bi len ei T := AfterBlock (fun xs => P xs \/ ~InBlockX bi len xs) s bi len ei T.
+Definition DuringBlock' (P: _ -> Prop) s bi len ei T :=
   forall t0 t1 a' s'
-    (XP: exec_prog p ((Addr a', s')::t1++t0))
-    (SO: ostartof t1 = Some (Addr (ei*4), s))
-    (CB: ContainsBlock p b s (Z.of_N bi))
-    (IB: Forall (InBlockX bi (length b)) ((Addr a', s')::t1)),
+    (XP: exec_prog arm_prog ((Addr a', s')::t1++(Addr (ei*4), s)::t0))
+    (T1: Forall T t1)
+    (IB: Forall (InBlockX bi len) ((Addr a', s')::t1++(Addr (ei*4), s)::nil)),
     P (Addr a', s').
-Lemma db_db': forall P b p s bi ei, DuringBlock P b p s bi ei <-> DuringBlock' P b p s bi ei.
+Lemma db_db': forall P s bi len ei T, DuringBlock P s bi len ei T <-> DuringBlock' P s bi len ei T.
 Proof.
   intros. unfold DuringBlock, DuringBlock', AfterBlock. split.
-    intros. apply H in XP. destruct XP. easy. now inversion IB. easy. easy. now inversion IB.
-    intros. destruct (inblockx_dec bi (length b) (Addr a', s')).
-      apply H in XP. now left. easy. easy. constructor. easy. easy.
+    intros. apply H in XP. destruct XP. easy. now inversion IB. easy. now inversion IB.
+    intros. destruct (inblockx_dec bi len (Addr a', s')).
+      apply H in XP. now left. easy. constructor. easy. easy.
       now right.
 Qed.
 
-(* the given block does not change as long as we are still in the block
-
-   note that we use DuringBlock instead of AfterBlock,
-   since we need to assume this property to prove that blocks go to a safe destination,
-   but to prove that the block is maintained even after exiting the block,
-   we need to know that indirect jumps always load from the table *)
-Definition MaintainsBlock p b bi ei s :=
-  DuringBlock (fun xs => ContainsBlock p b (snd xs) (Z.of_N bi)) b p s bi ei.
+Definition MaintainsBlock b bi ei s :=
+  ContainsBlock b s (Z.of_N bi) /\ DuringBlock (fun xs => ContainsBlock b (snd xs) (Z.of_N bi)) s bi (length b) ei (fun _ => True).
 
 Lemma containsblock_cons:
-  forall p b b' s i, ContainsBlock p (b::b') s i -> ContainsBlock p b' s (i+1).
+  forall b b' s i, ContainsBlock (b::b') s i -> ContainsBlock b' s (i+1).
 Proof.
   intros. unfold ContainsBlock, InBlock. intros. specialize (H i').
   rewrite <-(Z.add_simpl_r i 1) in H at 2.
@@ -132,32 +174,28 @@ Proof.
   simpl. destruct a. easy. intros. now rewrite startof_cons.
 Qed.
 Lemma ostartof_last{A}:
-  forall a (b:A), ostartof a = Some b -> exists c, a = c ++ [b].
+  forall a (b:A), ostartof a = Some b -> exists c, a = c ++ b::nil.
 Proof.
   destruct a. easy. intros. destruct (@exists_last _ (a::a0)). easy. destruct s. exists x. rewrite e, ostartof_niltail in H. inversion H. now rewrite <-H1.
 Qed.
 Lemma single_element{A}:
   forall (a: A) b c,
-    [a] = b ++ [c] ->
+    a::nil = b ++ c::nil ->
     a = c.
 Proof.
   intros. destruct b; simpl in H; inversion H; auto. now apply app_cons_not_nil in H2.
 Qed.
 Lemma forall_last{A}:
   forall (P: A -> Prop) y x1 t1 t2 x2,
-    y::x1::t1 = t2 ++ [x2] ->
+    y::x1::t1 = t2 ++ x2::nil ->
     Forall P (x1::t1) ->
     P x2.
 Proof.
-  intros. destruct (exists_last (ltac:(discriminate):x1::t1<>[])) as [? [? ?]].
+  intros. destruct (exists_last (ltac:(discriminate):x1::t1<>nil)) as [? [? ?]].
   rewrite e, app_comm_cons, app_inj_tail_iff in H. destruct H. subst.
   rewrite e, Forall_app in H0. destruct H0. now inversion H0.
 Qed.
 
-
-(* if there is at least one element in l where P holds,
-   we can split l into two lists where the first does not have any such element,
-   and the second list starts with one *)
 Lemma exsplit{A}{P: A -> Prop}:
   (forall a, {P a}+{~P a}) ->
   forall l, Exists P l -> exists l1 x l2, l = l1 ++ x :: l2 /\ P x /\ ~(Exists P l1).
@@ -170,8 +208,8 @@ Proof.
       apply IHl in H as [? [? [? [? [? ?]]]]]. rewrite H. exists (a::x), x0, x1. repeat split; auto.
       rewrite Exists_cons. unfold not. now rewrite Decidable.not_or_iff.
 Qed.
-Lemma cons_cons{A}: forall (a:A) b c, a::b::c = [a;b]++c. Proof. easy. Qed.
-Lemma app_cons{A}: forall (a:A) b c, c++a::b = (c++[a])++b.
+Lemma cons_cons{A}: forall (a:A) b c, a::b::c = (a::b::nil)++c. Proof. easy. Qed.
+Lemma app_cons{A}: forall (a:A) b c, c++a::b = (c++a::nil)++b.
 Proof.
   intros. now rewrite <-app_assoc, <-app_comm_cons, app_nil_l.
 Qed.
@@ -183,62 +221,28 @@ Proof.
   intros. destruct x. exists b. now subst.
 Qed.
 
-(* if the initial store does not matter,
-   we only need to consider traces that do not contain the entry more than once to prove AfterBlock *)
-Lemma afterblock_noloop:
-  (forall P b p s bi ei,
-    (forall t0 t1 t2 t3 t4 a' s0 s'
-      (* the trace through the block does not loop back to the entry *)
-      (NL: ~ Exists (fun x => fst x = Addr (ei*4)) t1)
-      (* the store we start with is reachable by some trace through the block *)
-      (RA: s = s0 \/ (Forall (InBlockX bi (length b)) t3 /\ exec_prog p (t4++(Addr (ei*4), s0)::t3++(Addr (ei*4), s)::t2)))
-
-      (XP: exec_prog p ((Addr a', s')::t1++(Addr (ei*4), s0)::t0))
-      (CB: ContainsBlock p b s (Z.of_N bi))
-      (IB: Forall (InBlockX bi (length b)) t1),
-      P (Addr a', s')) ->
-    AfterBlock P b p s bi ei)%N.
+Definition Reachable i' s' i s bi len :=
+  exists t,
+    let tt := (Addr (i'*4), s')::t++(Addr (i*4), s)::nil in
+    exec_prog arm_prog tt /\
+    Forall (InBlockX bi len) tt.
+Lemma afterblock_nol:
+  forall P s bi len ei,
+  (forall s', s = s' \/ Reachable ei s' ei s bi len ->
+  AfterBlock P s' bi len ei (fun t => fst t <> Addr (ei *4))) ->
+  AfterBlock P s bi len ei (fun _ => True).
 Proof.
-  intros. unfold AfterBlock. intros.
+  intros. unfold AfterBlock. intros. 
   assert (forall x: exit * store, {fst x = Addr (ei*4)} + {fst x <> Addr (ei*4)}) by repeat decide equality.
   destruct (Exists_dec _ t1 X).
   - apply (exsplit X) in e as [? [? [? [? [? ?]]]]]. apply undofst in H1 as [? ?]. subst.
-      rewrite <-app_assoc in XP. apply Forall_app in IB as [? ?].
-      rewrite ostartof_app in SO. apply ostartof_last in SO as [? ?]. destruct x0.
-      + inversion H3. eapply (H t0 x nil nil nil). apply H2. now left. subst. apply XP. assumption. assumption.
-      + rewrite H3 in XP. eapply H. apply H2. right. inversion H3. subst.
-        rewrite <-app_assoc, app_comm_cons in XP. split. inversion H1. apply Forall_app in H7 as [? ?]. apply H7.
-        apply XP. inversion H3. subst. apply XP. assumption. assumption.
-  - apply ostartof_last in SO as [? ?]. subst. exfalso. apply n. apply Exists_app. right. now constructor.
-Qed.
-Lemma afterblock_impl:
-  forall P Q p b s bi ei
-    (I: forall x, P x -> Q x)
-    (AB: AfterBlock P p b s bi ei),
-    AfterBlock Q p b s bi ei.
-Proof.
-  unfold AfterBlock. intros. apply I. eapply AB. apply XP. all: easy.
-Qed.
-
-Lemma afterblock_suffix{P b p s bi ei ei' s' t0 t2}:
-  forall t1
-    (AB: AfterBlock P b p s bi ei)
-    (XP: exec_prog p (t2++(Addr (ei'*4), s')::t1++t0))
-    (SO: ostartof t1 = Some (Addr (ei * 4), s))
-    (CB: ContainsBlock p b s (Z.of_N bi))
-    (IB: Forall (InBlockX bi (length b)) t1),
-    AfterBlock P b p s' bi ei'.
-Proof.
-  intros; unfold AfterBlock; intros.
-  eapply (AB t0 (t4++t1)).
-  - rewrite <-app_assoc, app_comm_cons. rewrite app_cons in XP. apply exec_prog_split in XP as [? [? ?]]. apply exec_prog_app.
-      easy.
-      unfold can_step_between in *. destruct app eqn:e; auto. erewrite ostartof_some_cons. rewrite ostartof_niltail in H0. apply H0.
-      easy.
-      rewrite app_comm_cons in XP0. now apply exec_prog_split in XP0.
-  - apply ostartof_last in SO as [? ?]. now rewrite H, app_assoc, ostartof_niltail.
-  - now destruct t4.
-  - now rewrite Forall_app.
+    assert (XP':=XP).
+    apply exec_prog_tail in XP. rewrite <-app_assoc in XP. apply exec_prog_split in XP as [XP _].
+    rewrite app_cons in XP. apply exec_prog_split in XP as [_ [_ XP]].
+    eapply H. right. exists x1. split. apply XP. now rewrite <-app_assoc, Forall_app in IB.
+    rewrite app_comm_cons in XP'. apply exec_prog_split in XP' as [_ [_ XP']]. apply XP'. now apply Forall_Exists_neg. apply Forall_app in IB as [IB _].
+    apply Forall_app in IB as [? ?]. apply Forall_app. split. easy. constructor. now inversion H1. easy.
+  - eapply H. now left. apply XP. now apply Forall_Exists_neg. easy.
 Qed.
 Lemma xp_splice:
   forall p t t' x, exec_prog p (x::t) -> exec_prog p t' -> ostartof t' = Some x -> exec_prog p (t'++t).
@@ -246,121 +250,53 @@ Proof.
   intros. apply exec_prog_app. now apply exec_prog_tail in H. unfold can_step_between. destruct t. easy. rewrite H1. now inversion H. easy.
 Qed.
 
-(* for a block b that is maintained through the entire execution through b, where the instruction at our entry index is z, if
-      1) z falls through to z' inside the block, P is true for this step, and P always holds after executing from z'
-      2) z goes to a state outside the block where P holds
-   or 3) z raises an exception
-   then P always holds after b if we start at z *)
 Lemma afterblock_step:
-  forall p b z s bi ei P
-    (MB: MaintainsBlock p b bi ei s)
+  forall b z s bi ei P T
+    (MB: MaintainsBlock b bi ei s)
     (E: bi <= ei)
     (Z: nth_error b (Z.to_nat (Z.of_N ei - Z.of_N bi)) = Some z),
-    (forall c' s s' x, exec_stmt armc s (arm2il (ei*4) (arm_decode z)) c' s' x ->
-      (* case 1 *)
+    (forall c' s' x, exec_stmt armc s (arm2il (ei*4) (arm_decode z)) c' s' x ->
         (x = None /\
-        (MaintainsBlock p b bi (ei+1) (reset_temps s s') -> AfterBlock P b p (reset_temps s s') bi (ei+1)) /\
+        (MaintainsBlock b bi (ei+1) (reset_temps s s') -> 
+          Reachable (ei+1) (reset_temps s s') ei s bi (length b) ->
+          AfterBlock P (reset_temps s s') bi (length b) (ei+1) T) /\
         P (Addr ((ei+1)*4), (reset_temps s s'))) \/
-      (* case 2 (fallthru) *)
         (x = None /\
-        length b = 1%nat /\
+        length b = N.to_nat (ei - bi + 1) /\
         P (Addr ((ei+1)*4), (reset_temps s s'))) \/
-      (* case 2 (jump) *)
         (exists a, x = Some (Addr a) /\
         P (Addr a, (reset_temps s s')) /\
-        ~ (InBlock (Z.of_N bi) (length b) a)) \/
-      (* case 3 *)
+        (~ (InBlock (Z.of_N bi) (length b) a) \/ ~ T (Addr a, (reset_temps s s')))) \/
         (exists a, x = Some (Raise a))) ->
-    AfterBlock P b p s bi ei.
+    AfterBlock P s bi (length b) ei T.
 Proof.
   intros. unfold AfterBlock. intros.
+  destruct MB as [CB MB].
   specialize (CB ei) as CB'. rewrite Z in CB'.
   remember (Z.to_nat _). pose proof (proj1 (nth_error_Some b n) ltac:(now rewrite Z)).
   assert (InBlock (Z.of_N bi) (length b) (ei*4)) as IB' by (split; [lia|now exists ei]).
   specialize (CB' IB').
-  apply ostartof_last in SO as [? ?]. rewrite H1, 2 app_comm_cons in XP.
-  destruct (@exists_last _ ((Addr a', s')::x) ltac:(discriminate)) as [? [? ?]]. rewrite e, <-2app_assoc in XP.
-  assert (XP':=XP). apply exec_prog_split in XP as [XP _]. simpl in XP.
-  inversion XP. inversion H4. rewrite CB' in LU. inversion LU. subst. apply H in XS.
-  clear H4 H5 LU H. destruct XS as [[? [? ?]]|[[? [? ?]]|[[? [? [? ?]]]|[? ?]]]]; subst;
-    (destruct x; [ apply single_element in e; inversion e; now try rewrite N.mul_add_distr_r in H2|]).
+  destruct (@exists_last _ ((Addr a', s')::t1) ltac:(discriminate)) as [? [? ?]]. rewrite app_comm_cons, e, <-app_assoc in XP. simpl in XP.
+  assert (XP':=XP). apply exec_prog_split in XP as [XP _].
+  inversion XP. inversion H3. rewrite CB' in LU. inversion LU. subst. apply H in XS.
+  clear H4 LU H. destruct XS as [[? [? ?]]|[[? [? ?]]|[[? [? [? ?]]]|[? ?]]]]; subst;
+    (destruct x; [ inversion e; now try rewrite N.mul_add_distr_r in H2|]).
   {
-    eapply H1.
-    eapply (afterblock_suffix [_] MB); [ rewrite N.mul_add_distr_r, app_nil_l; apply XP | now try constructor .. ].
-    rewrite app_assoc, <-e in XP'. simpl in XP'. rewrite app_comm_cons in XP'. apply XP'.
-    now erewrite <-ostartof_app, <-app_cons, app_nil_l, e, ostartof_app, N.mul_add_distr_r.
-    apply db_db' in MB. eapply MB; [rewrite <-app_cons, app_nil_l; apply XP| auto .. ];
-      apply (forall_last (InBlockX bi (length b))) in e;
-        [apply (Forall_cons _ e); constructor; now try apply IB'|].
-    all: now apply Forall_app in IB.
+    inversion e; subst; simpl in XP'.
+    eapply H1. 
+      pose proof (exec_prog_step _ _ _ (exec_prog_none _ _) H3).
+      rewrite <-app_assoc, Forall_app in IB. destruct IB.
+      split. apply db_db' in MB. eapply MB. rewrite app_nil_l. apply H. easy. easy.
+      intros ???????. eapply MB. rewrite app_cons,app_comm_cons in XP0. apply exec_prog_split in XP0 as [_ [_ ?]].
+      eapply (xp_splice _ _ _ _ H H6). now rewrite app_comm_cons, ostartof_niltail, N.mul_add_distr_r. now apply Forall_forall.
+      apply Forall_app. split. easy. now apply Forall_app in H5.
+      exists nil. split. simpl. apply exec_prog_step. apply exec_prog_none. now rewrite N.mul_add_distr_r.
+      rewrite <-app_assoc in IB. simpl in *. rewrite Forall_app in IB. now rewrite N.mul_add_distr_r.
+    rewrite N.mul_add_distr_r. apply XP'. now apply Forall_app in T1.
+    apply Forall_app in IB. now rewrite N.mul_add_distr_r.
   }
-  all: apply (forall_last (InBlockX bi (length b))) in e;
-    unfold InBlockX, InBlock in e; simpl in e; [now try lia|now apply Forall_app in IB].
-Qed.
-
-(* like afterblock_step, but we can forget about the first instruction of the block *)
-Lemma afterblock_cons:
-  forall p b b' s i P
-    (MB: MaintainsBlock p (b::b') i i s),
-    (forall c' s s' x, exec_stmt armc s (arm2il (i*4) (arm_decode b)) c' s' x ->
-      (* case 1 *)
-        (x = None /\
-        (MaintainsBlock p b' (i+1) (i+1) (reset_temps s s') -> AfterBlock P b' p (reset_temps s s') (i+1) (i+1)) /\
-        P (Addr ((i+1)*4), (reset_temps s s'))) \/
-      (* case 2 (fallthru) *)
-        (x = None /\
-        b' = nil /\
-        P (Addr ((i+1)*4), (reset_temps s s'))) \/
-      (* case 2 (jump) *)
-        (exists a, x = Some (Addr a) /\
-        P (Addr a, (reset_temps s s')) /\
-        ~ (InBlock (Z.of_N i) (length (b::b')) a)) \/
-      (* case 3 *)
-        (exists a, x = Some (Raise a))) ->
-    AfterBlock P (b::b') p s i i.
-Proof.
-  (* todo: clean this proof up *)
-  intros. apply afterblock_noloop.
-  intros. assert (XP':=XP). assert(CB':=CB). rewrite app_comm_cons in XP.
-  remember (_::t1). destruct (@exists_last _ l ltac:(now subst)) as [? [? ?]]. subst.
-  rewrite e, <-app_assoc in XP. simpl in XP. apply exec_prog_split in XP as [XP _]. inversion XP. clear x1 l H3 H0 H1. inversion H2. clear H2. subst.
-  assert (Some(sz, q) = p s (i*4)).
-  { destruct RA. now rewrite H0. destruct H0. unfold MaintainsBlock, DuringBlock in MB. specialize (MB t2 (t3++[(Addr (i*4), s)])).
-    simpl in MB. rewrite <-app_assoc in MB. simpl in MB. apply exec_prog_split in H1 as [? _]. eapply MB in H1. shelve. now rewrite ostartof_niltail. easy. apply Forall_app. split. easy. constructor. apply inblock_start. easy. Unshelve. destruct H1.
-    specialize (CB i (inblock_start)). specialize (H1 i (inblock_start)). rewrite Z.sub_diag, nth_error_O in CB, H1. simpl in CB, H1. now rewrite <-LU, H1, CB. exfalso.  apply H1. apply inblock_start.
-    }
-  specialize (CB i (inblock_start )). rewrite Z.sub_diag, nth_error_O in CB. simpl in CB. rewrite CB in H0. inversion H0.
-  subst. apply H in XS. destruct XS as [?|[?|[?|?]]].
-  shelve.
-  - destruct H1 as [? [? ?]]. destruct t1. apply single_element in e. inversion e. subst. rewrite H5. now rewrite N.mul_add_distr_r in H3.
-    apply forall_last with (P:=InBlockX i (length (b::b'))) in e.
-    subst. simpl in e. unfold InBlockX in e. simpl in e. unfold InBlock in e. lia. easy.
-  - destruct H1 as [? [? [? ?]]]. destruct t1. apply single_element in e. inversion e. subst. now rewrite H5.
-    apply forall_last with (P:=InBlockX i (length (b::b'))) in e.
-    subst. simpl in e. unfold InBlockX in e. simpl in e. contradiction. easy.
-  - destruct H1. subst. destruct t1. apply single_element in e. easy.
-    apply forall_last with (P:=InBlockX i (length (b::b'))) in e. easy. easy.
-    Unshelve.
-    destruct H1 as [? [? ?]].
-
-
-    destruct t1. apply single_element in e. inversion e. rewrite H5. subst. simpl.  rewrite N.mul_add_distr_r in H3. easy.
-    subst; simpl in *. eapply H2. shelve. rewrite 2 app_comm_cons in XP'. apply XP'. now erewrite <-ostartof_app, <-app_cons, app_nil_l, e, ostartof_app, N.mul_add_distr_r. rewrite N2Z.inj_add. eapply containsblock_cons. remember (_::_::_). replace l with
-      ([(Addr (i * 4 + 4), reset_temps s0 s'0) ; (Addr (i * 4), s0)] ++ t0)%N in XP. destruct RA. apply db_db' in MB. eapply MB. apply XP. now rewrite e0. easy. 
-      apply forall_last with (P:=InBlockX i (length (b::b'))) in e. constructor. assumption. constructor. apply inblock_start. easy. assumption. apply db_db' in MB. eapply MB.
-      destruct a. apply exec_prog_split in e0 as [? _]. apply exec_prog_split in XP as [_ [_ ?]]. 
-
-      enough (exec_prog p (([(Addr (i * 4 + 4), reset_temps s0 s'0);(Addr (i * 4), s0)]++t3++[(Addr (i*4), s)])++t2)). apply H5. rewrite <-app_assoc.
-      apply exec_prog_app. rewrite <-app_cons. now apply exec_prog_tail in H1. unfold can_step_between. simpl. rewrite <-app_assoc. destruct app; auto. now inversion H1. easy. simpl. now rewrite startof_niltail. assumption.
-    apply forall_last with (P:=InBlockX i (length (b::b'))) in e. constructor. easy. constructor. apply inblock_start. apply Forall_app. split. easy. constructor. apply inblock_start. easy. easy.
-      eapply Forall_impl. replace (length b') with ((length (b::b'))-1)%nat. apply inblockx_s. simpl. lia. apply Forall_Exists_neg in NL. now apply Forall_and.
-      Unshelve.
-      clear H NL CB H0 H2 H3 LU. apply db_db'. apply db_db' in MB. unfold DuringBlock', DuringBlock in *. intros. rewrite N2Z.inj_add. eapply containsblock_cons.
-      destruct RA; eapply MB; rewrite app_comm_cons in XP0; apply exec_prog_split in XP0 as [_ [_ ?]]; pose proof (xp_splice _ _ _ _ XP H); eapply ostartof_some_cons in SO; rewrite N.mul_add_distr_r in SO; apply H0 in SO. rewrite <-app_comm_cons, app_cons in SO. apply SO. now rewrite ostartof_niltail, e0. assumption.
-      rewrite app_comm_cons, Forall_app. split. eapply Forall_impl in IB0. apply IB0. apply inblockx_cons. constructor. apply inblock_start. easy.
-      destruct a. apply exec_prog_split in e0 as [? _]. rewrite <-app_comm_cons, app_cons , app_comm_cons in SO. apply exec_prog_split in SO as [_ [_ ?]].  pose proof (xp_splice _ _ _ _ H1 H2). rewrite app_comm_cons, ostartof_niltail, <-app_comm_cons, (app_cons (_, s)) in H3. 
-      rewrite <-app_comm_cons, (app_assoc (t6++_)) in H3. apply (H3 eq_refl). now rewrite app_assoc, ostartof_niltail. assumption. constructor.
-      apply inblockx_cons. now inversion IB0. repeat (rewrite Forall_app; split). eapply Forall_impl. apply inblockx_cons. now inversion IB0. constructor. apply inblock_start. easy. easy. constructor. apply inblock_start. easy.
+  all: try destruct H2; inversion e; subst; apply Forall_app in IB as [IB _], IB as [_ IB], T1 as [_ T1]; inversion IB; subst;
+    unfold InBlockX, InBlock in *; simpl in *; now (lia || inversion T1).
 Qed.
 
 Definition SafeDestX i2i' pol ai si ilen (xs: exit * store) :=
@@ -368,6 +304,7 @@ Definition SafeDestX i2i' pol ai si ilen (xs: exit * store) :=
   | Addr a => SafeDest i2i' pol ai si ilen a
   | _ => False
   end.
+
 
 
 Lemma forget_cond:
@@ -381,6 +318,19 @@ Proof.
       apply XS1.
       inversion XS0. destruct b; [apply XIf with (b:=0)|apply XIf with (b:=1)]; now try constructor.
 Qed.
+Local Ltac mystep H := match type of H with ?a => idtac a end; match type of H with 
+                       | context[N.mul ?a 4] => remember (N.mul a 4); mystep H
+                       | context[scast ?a ?b ?c] =>
+                           remember (scast a b c); mystep H
+                       | context[if ?a then ?b else ?c] => destruct a eqn:e; try lia
+                       | exec_stmt _ _ (arm2il _ _) _ _ _ =>
+                           cbv[arm2il arm_cond_il arm_b_il BranchWritePC arm_R arm_bfx_il] in H; mystep H
+                       | exec_stmt _ _ (_ $; If (arm_cond_exp (Z.to_N Z14)) _ _) _ _ _ =>
+                           simpl (Z.to_N Z14) in H; cbv[arm_cond_exp] in H; simpl (if _:bool then _ else _) in H
+                       | exec_stmt _ _ (_ $; If (arm_cond_exp _) _ _) _ _ _ => apply forget_cond in H; mystep H
+                       | exec_stmt _ _ _ _ _ _ => step_stmt H
+                       | _ /\ True => destruct H as [H _]; mystep H
+                       end.
 
 Ltac destruct_match_in H :=
   repeat match type of H with context[match ?x with _ => _ end] =>
@@ -399,6 +349,16 @@ Lemma arm_assemble_all_first:
 Proof.
   induction z. intros. unfold arm_assemble_all in H. destruct_match_in H; discriminate. intros. exists a0, z. repeat split; unfold arm_assemble_all in H; destruct_match_in H; try discriminate. inversion H. now subst. apply arm_assemble_eq in e. inversion H. now subst.
 Qed.
+Lemma arm_assemble_all_app:
+  forall a b z, arm_assemble_all (a++b) = Some z ->
+  exists a' b', z = a'++b' /\ arm_assemble_all a = Some a' /\ arm_assemble_all b = Some b'.
+Proof.
+  induction a. exists nil, z. easy.
+  intros. simpl in H. destruct_match_in H; try discriminate.
+  apply IHa in e0 as [? [? [? [? ?]]]]. exists (z0::x), x0. repeat split.
+  inversion H. now subst. 
+  simpl. now rewrite e, H1. easy.
+Qed.
 Lemma arm_assemble_all_len:
   forall a b, arm_assemble_all a = Some b -> length a = length b.
 Proof.
@@ -409,73 +369,386 @@ Lemma arm_assemble_all_cond_len:
 Proof.
   intros. unfold arm_assemble_all_cond in H. destruct Z.ltb. apply arm_assemble_all_len in H. rewrite <- H. simpl. lia. apply arm_assemble_all_eq in H. rewrite <- H, length_map. lia.
 Qed.
+Lemma update_cancel2: forall (s:store) v n v' n' n0,
+  v <> v' -> s[v' := n0][v := n][v' := n'] = s[v' := n'][v := n].
+Proof.
+  intros. now rewrite update_swap, update_cancel by easy.
+Qed.
+
+Lemma aaa: forall a b c m, b mod m = c mod m -> (a + b) mod m = (a + c) mod m.
+Proof.
+  intros. now rewrite N.Div0.add_mod, H, <-N.Div0.add_mod.
+Qed.
+Lemma add: forall i s s' c' x reg imm shift,
+  (reg < 15)%Z ->
+  (imm < 2^8) ->
+  (shift < 2^4) ->
+  exec_stmt armc s (arm2il i (ARM_data_i ARM_ADD 14 0 reg reg (Z.lor (Z.shiftl (Z.of_N shift) 8) (Z.of_N imm)))) c' s' x ->
+  reset_temps s s' = s[R_PC := i] [arm_varid (Z.to_N reg) := (s (arm_varid (Z.to_N reg)) ⊕ (imm >> (2 * shift) .| ((imm << (32 - (2* shift))) mod 2^ 32)))]
+  /\ x = None.
+Proof.
+  intros.
+  cbv[arm2il arm_data_i_il arm_data_op_il arm_data_i_addwcarry ARMExpandImm_C AddWithCarry arm_data_il arm_cond_il Shift_C] in H2.
+  simpl (Z.to_N 0 =? 1) in H2.
+  destruct N.eqb eqn:e; try lia. simpl (Z.to_N 14) in H2. cbv[arm_cond_exp] in H2. cbv[N.ltb N.compare Pos.compare Pos.compare_cont andb arm_assign_R] in H2.
+  remember (xbits _ _ _).
+  remember (2 * (xbits _ _ _)).
+  rewrite Z2N_inj_lor, Z2N_inj_shiftl, N2Z.id, xbits_lor, xbits_shiftl in Heqn, Heqn0 by (try apply Z.shiftl_nonneg; lia).
+  rewrite xbits_0_j, N.shiftl_0_l, N.lor_0_l, N2Z.id, xbits_0_i, N.mod_small in Heqn by assumption.
+  rewrite xbits_0_i, N.mod_small, N2Z.id, xbits_above, N.lor_0_r, N.shiftl_0_r in Heqn0 by assumption.
+  unfold arm_varid. destruct_match_eqn; try lia; cbv[arm_varid arm_R N.eqb] in H2;
+  step_stmt H2; destruct H2 as [H2 _]; step_stmt H2; destruct H2 as [[H2 H3] _];
+  (split; [clear H3|apply H3]);
+  rewrite H2; subst;
+  rewrite N.add_0_r, msub_sub, (N.mod_small (_ - _)) by lia;
+  (erewrite <-(N.mod_small (_ >> _)), <-N_lor_mod_pow2, N.Div0.add_mod_idemp_r, N.Div0.mod_mod; [reflexivity|
+  assert ((imm >> 2 * shift) <= imm) by apply N.shiftr_upper_bound; lia]).
+Qed.
+
+Lemma rt:
+  forall s s' n, reset_temps s s' (arm_varid n) = s' (arm_varid n).
+Proof.
+  intros. unfold arm_varid. now destruct_match_eqn.
+Qed.
+Lemma reset_temps_models{s s'}:
+  models armc s' -> models armc (reset_temps s s').
+Proof.
+  unfold models. intros. unfold reset_temps, reset_vars, archtyps. rewrite CV. now apply H.
+Qed.
+Lemma Nshiftl_add_distr : forall a b s, (a << s) + (b << s) = (a + b) << s.
+Proof.
+  intros. now rewrite !N.shiftl_mul_pow2, N.mul_add_distr_r.
+Qed.
+
+Local Ltac replace_nth a := match goal with |- nth_error _ ?n = _ => replace n with a by lia end.
+Lemma reachablecat{i2 s2 i1 s1 i0 s0 bi len}:
+  forall
+    (R: Reachable i2 s2 i1 s1 bi len)
+    (R': Reachable i1 s1 i0 s0 bi len),
+    Reachable i2 s2 i0 s0 bi len.
+Proof.
+  intros. destruct R as [? [?]], R' as [? [?]].
+  pose proof (xp_splice _ _ _ _ H1 H ltac:(now rewrite app_comm_cons, ostartof_niltail)).
+  simpl in H3. eexists. split. rewrite app_assoc in H3. apply H3. rewrite <-app_assoc, app_comm_cons, Forall_app. split. easy. now inversion H2.
+Qed.
+Local Ltac r :=
+  repeat match goal with
+         | [ H: Reachable _ _ ?i ?s ?bi ?len, H1: Reachable ?i ?s _ _ ?bi ?len |- _ ] =>
+             let r := fresh "r" in
+             pose proof (reachablecat H H1) as r; clear H H1; rename r into H1
+         end.
+
+Lemma reset_temps_overwrite_l: forall s1 s2 s3, reset_temps (reset_temps s1 s2) s3 = reset_temps s1 s3.
+Proof. now specialize (reset_vars_overwrite_l armc). Qed.
+Lemma reset_temps_overwrite_r: forall s1 s2 s3, reset_temps s1 (reset_temps s2 s3) = reset_temps s1 s3.
+Proof. now specialize (reset_vars_overwrite_r armc). Qed.
+Lemma reset_temps_update_l:
+  forall s s' n v v', reset_temps (s[R_PC := v][arm_varid n := v']) s' = reset_temps s s'.
+Proof.
+  intros. unfold reset_temps, arm_varid. now rewrite reset_vars_fchoose, !fchoose_update_l by now destruct_match_eqn. 
+Qed.
+Lemma reset_temps_not_temp:
+  forall v s s', armc v <> None -> reset_temps s s' v = s' v.
+Proof.
+  intros. unfold reset_temps. rewrite reset_vars_fchoose. unfold fchoose. destruct in_ctx eqn:e. easy. unfold in_ctx in e. now destruct_match_in e.
+Qed.
+Require Import FunctionalExtensionality.
+Lemma reset_temps_id:
+  forall s, reset_temps s s = s.
+Proof.
+  intros. unfold reset_temps, reset_vars. apply functional_extensionality. intro. now destruct (archtyps x).
+Qed.
+Lemma reset_temps_revert: forall s s', reset_temps s' (reset_temps s s') = s'.
+Proof. now specialize (reset_vars_revert armc). Qed.
+Lemma after_arm_add: forall P reg v s bi b pre post T ei
+  (MB: MaintainsBlock b bi ei s)
+  (M: models armc s)
+  (E: ei = bi + N.of_nat (length pre))
+  (B: arm_assemble_all (pre++arm_add reg (Z.of_N v)++post) = Some b)
+  (L: (0 < length post)%nat)
+  (R: (reg < 15)%Z)
+  (I: bi + N.of_nat (length pre) + 3 < 2 ^ 30)
+  (IB: (forall x, InBlockX bi (length b) x -> P x))
+  (PC: forall s',
+    MaintainsBlock b bi (ei+4) s' ->
+    Reachable (ei+4) s' ei s bi (length b) ->
+    models armc s' ->
+    reset_temps s s' = s[R_PC := (ei + 3) * 4][arm_varid (Z.to_N reg) := s (arm_varid (Z.to_N reg)) ⊕ v] ->
+    AfterBlock P s' bi (length b) (ei+4) T),
+  AfterBlock P s bi (length b) ei T.
+Proof.
+  intros. unfold arm_add, Z4, Z8, Z12, Z14, Z16, Z24, Z32 in B. cbn[app]in B. rewrite !zxbits_eq in B.
+
+  apply arm_assemble_all_app in B as [b_pre [b_tail [? [BPRE B]]]]; subst; rename b_tail into b.
+  apply arm_assemble_all_len in BPRE.
+  apply arm_assemble_all_first in B as [? [? [? [? ?]]]]; subst.
+  eapply afterblock_step. easy. lia. 
+  replace_nth (length pre). rewrite nth_error_app2 by lia. replace_nth O. reflexivity.
+
+  intros.
+  epose proof (reset_temps_models (pres_frame_exec_stmt M M _ H0)) as M'.
+  rewrite H1, <-(Z2N.id 4), <-(Z2N.id (Z_xbits _ _ _)) in H0 by (apply Z_xbits_nonneg||lia).
+  apply add in H0 as [? ?]; [|assumption|rewrite Z2N_xbits by lia; apply xbits_bound|lia]. 
+  left; repeat split; [easy|intros ? RA|shelve].
+
+  apply arm_assemble_all_first in H as [? [? [? [? ?]]]]; subst x1.
+  eapply afterblock_step. easy. lia.
+replace_nth (S(length pre)). rewrite nth_error_app2. replace_nth 1%nat. now subst. lia.
+
+  intros.
+  epose proof (reset_temps_models (pres_frame_exec_stmt M' M' _ H2)) as M''.
+  rewrite H5, <-(Z2N.id 8), <-(Z2N.id (Z_xbits _ _ _)) in H2 by (apply Z_xbits_nonneg||lia).
+  apply add in H2 as [? ?]; [|assumption|rewrite Z2N_xbits by lia; apply xbits_bound|lia]. 
+  left; repeat split; [easy|intros|shelve]. r.
+
+  apply arm_assemble_all_first in H as [? [? [? [? ?]]]]; subst x3.
+  eapply afterblock_step. easy. lia.
+  replace_nth (length pre + 2)%nat. rewrite nth_error_app2. replace_nth 2%nat. now subst. lia.
+
+  intros.
+  epose proof (reset_temps_models (pres_frame_exec_stmt M'' M'' _ H8)) as M'''.
+  rewrite H9, <-(Z2N.id 12), <-(Z2N.id (Z_xbits _ _ _)) in H8 by (apply Z_xbits_nonneg||lia).
+  apply add in H8 as [? ?]; [|assumption|rewrite Z2N_xbits by lia; apply xbits_bound|lia]. 
+  left; repeat split; [easy|intros|shelve]. r.
+
+  apply arm_assemble_all_first in H as [? [? [? [? ?]]]]; subst x5.
+  eapply afterblock_step. easy. lia.
+  replace_nth (length pre + 3)%nat. rewrite nth_error_app2. replace_nth 3%nat. now subst. lia.
+
+  intros.
+  epose proof (reset_temps_models (pres_frame_exec_stmt M''' M''' _ H12)) as M''''.
+  rewrite H13 in H12.
+  replace (Z_xbits (Z.of_N v) 0 8) with (Z.lor (Z.shiftl (Z.of_N 0) 8) (Z_xbits (Z.of_N v) 0 8)) in H12 by now rewrite Z.lor_0_l.
+  rewrite <-(Z2N.id (Z_xbits _ _ _)) in H12 by (apply Z_xbits_nonneg||lia).
+  apply add in H12 as [? ?]; [|assumption|rewrite Z2N_xbits by lia; apply xbits_bound|lia]. 
+  left; repeat split; [easy|intros|shelve]. r.
+
+  rewrite <-3N.add_assoc. apply PC. now rewrite <-3N.add_assoc in H15.
+  now rewrite <-3N.add_assoc in RA. apply M''''.
+
+
+  unfold reset_temps in *.
+  rewrite !reset_vars_overwrite_l, !rt in *.
+  rewrite reset_vars_overwrite_r, H12, H8, H2, H0.
+  fold reset_temps in *.
+  assert (arm_varid (Z.to_N reg) <> R_PC) by (unfold arm_varid; destruct_match_eqn; lia || discriminate).
+  repeat rewrite update_swap, update_cancel by easy. rewrite <-2N.add_assoc.
+  remember ((s'1 _ + _) mod _). remember ((_ + _) mod _). enough (n = n0). now rewrite H17. subst.
+  rewrite <-(rt s), H8, update_updated, <-(rt s), H2, update_updated, <-(rt s), H0, update_updated.
+  rewrite ! N.Div0.add_mod_idemp_l, <-N.add_assoc, N.Div0.add_mod_idemp_l, <-!N.add_assoc.
+  Unshelve. shelve.
+  3,6,9,12: apply IB; unfold InBlockX, InBlock; simpl; apply arm_assemble_all_len in H; simpl in H; rewrite length_app; subst; simpl; split; [try lia| apply N.divide_factor_r].
+  all: try exact armc; apply welltyped_arm2il; lia.
+  Unshelve.
+  clear.
+  apply aaa. rewrite !Z2N_xbits by (apply N2Z.is_nonneg || lia). rewrite !N2Z.id. cbv [Z.to_N N.mul Pos.mul]. simpl N.sub. 
+  rewrite (N.shiftl_mul_pow2 _ 32), N.Div0.mod_mul, N.lor_0_r.
+  erewrite <-(N.mod_small (_>>8)), <-(N.mod_small (_>>16)), <-(N.mod_small (_>>24)), <-(N.mod_small (_>>0)), <-!N_lor_mod_pow2.
+  rewrite !N.add_assoc. repeat rewrite !N.Div0.add_mod_idemp_r, N.add_comm, !N.add_assoc.
+  apply N.bits_inj. intro. 
+  destruct (N.lt_ge_cases n (32)).
+  rewrite !N.mod_pow2_bits_low by assumption.
+  rewrite 3 shiftr_low_pow2, !N.lor_0_l. rewrite <-!lor_plus, !N.lor_spec.
+  rewrite !xbits_equiv, <-!N.ldiff_ones_r, !N.ldiff_spec, !N.shiftr_0_r, !N_ones_spec_ltb.
+  destruct (N.lt_ge_cases n 8).
+    repeat replace (_ <? _) with true by lia.
+    now rewrite !andb_false_r, N.mod_pow2_bits_low. 
+  destruct (N.lt_ge_cases n 16).
+    repeat replace (_ <? _) with true by lia. replace (_ <? _) with false by lia.
+    now rewrite !andb_false_r, N.mod_pow2_bits_low, N.mod_pow2_bits_high, andb_true_r, orb_false_r.
+  destruct (N.lt_ge_cases n 24).
+    replace (_ <? _) with true by lia. repeat replace (_ <? _) with false by lia.
+    now rewrite !andb_false_r, !andb_true_r, N.mod_pow2_bits_low, !N.mod_pow2_bits_high, !orb_false_r by easy.
+    repeat replace (_ <? _) with false by lia.
+    now rewrite N.mod_pow2_bits_low, !N.mod_pow2_bits_high, !andb_true_r, !orb_false_r by easy.
+  apply N.bits_inj_0. intro. rewrite N.land_spec. 
+  destruct (N.lt_ge_cases n0 24).
+    now rewrite N.shiftl_spec_low, andb_false_l by lia.
+    unfold xbits. now rewrite (N.shiftl_spec_high' _ 16), N.mod_pow2_bits_high, andb_false_r by lia.
+  apply N.bits_inj_0. intro. rewrite N.land_spec, andb_false_iff. 
+  destruct (N.lt_ge_cases n0 16).
+    change 24 with (8+16). rewrite <- N.shiftl_shiftl, Nshiftl_add_distr, N.shiftl_spec_low by easy. now left.
+    rewrite !xbits_equiv, N.shiftl_spec_high', N.shiftr_spec', N.mod_pow2_bits_high by lia. now right.
+  apply N.bits_inj_0. intro. rewrite N.land_spec, andb_false_iff. 
+  destruct (N.lt_ge_cases n0 8).
+    change 16 with (8+8). change 24 with (16+8). rewrite <-!N.shiftl_shiftl, !Nshiftl_add_distr, N.shiftl_spec_low by easy. now left.
+    unfold xbits. rewrite N.shiftr_0_r, N.mod_pow2_bits_high by lia. now right.
+     pose proof (xbits_bound v 8 16). simpl in H0. lia.
+     pose proof (xbits_bound v 16 24). simpl in H0. lia.
+     apply xbits_bound.
+     now rewrite !N.mod_pow2_bits_high by assumption.
+     pose proof (xbits_bound v 0 8). simpl in *. lia.
+     pose proof (xbits_bound v 8 16). pose proof (N.shiftr_upper_bound (xbits v 8 16) 24). simpl in H. lia.
+     pose proof (xbits_bound v 16 24). pose proof (N.shiftr_upper_bound (xbits v 16 24) 16). simpl in H. lia.
+     pose proof (xbits_bound v 24 32). pose proof (N.shiftr_upper_bound (xbits v 24 32) 8). simpl in H. lia.
+Qed.
+
+Lemma bfx_bound: forall i s s' c' x widthm1 rd lsb rn,
+  exec_stmt armc s (arm2il i (ARM_bfx false 14 (Z.of_N widthm1) rd lsb rn)) c' s' x ->
+  exists n, s' = s[R_PC := i][arm_varid (Z.to_N rd) := n] /\ n < 2 ^ (widthm1+1) /\ x = None.
+Proof.
+  (* intros. mystep H; unfold arm_varid in H; destruct_match_in H; simpl in H; cbv [arm_cond_exp arm_assign_R arm_varid] in H; simpl in H; destruct_match_in H; rewrite N2Z.id in H; remember (Z.to_N lsb); remember (n + _); step_stmt H; destruct H; inversion H; exists n1; repeat split; *)
+  (* inversion E; inversion E1; rewrite <-H6, <-H11; simpl; subst; replace (widthm1 + 1) with (N.succ (Z.to_N lsb + widthm1) - Z.to_N lsb) by lia; apply xbits_bound. *)
+Admitted.
+(**)
+Lemma UBFX_bound: forall i s s' c' x reg sl sr,
+  exec_stmt armc s (arm2il i (UBFX reg reg sl (Z.of_N sr))) c' s' x ->
+  (reg <> 15)%Z ->
+  (sr < 32) ->
+  exists n, s' = s[R_PC := i][arm_varid (Z.to_N reg) := n] /\ n < 2 ^ (32 - sr) /\ x = None.
+Proof.
+  intros. cbv [UBFX] in H. unfold Z31 in H. rewrite <-(Z2N.id 31) , <-N2Z.inj_sub in H by lia. apply bfx_bound in H. now rewrite <-N.add_sub_swap in H by lia.
+Qed.
+Lemma reachableduring {P s len bi ei i s'}: Reachable i s' ei s bi len -> DuringBlock P s bi len ei (fun _ => True) -> P (Addr (i*4), s').
+
+Proof.
+  intros. apply db_db' in H0. destruct H as [? [? ?]]. eapply H0. rewrite app_cons in H. rewrite app_nil_r in H. apply H. 
+  now apply Forall_forall.
+  easy.
+Qed.
+Lemma mt:
+  forall b bi ei s s'
+    (MB: MaintainsBlock b bi ei s)
+    (RA: Reachable ei s' ei s bi (length b)),
+    MaintainsBlock b bi ei s'.
+Proof.
+  unfold MaintainsBlock. intros. destruct MB. split.
+  eapply reachableduring in H0. simpl in H0. apply H0. apply RA.
+
+  unfold DuringBlock, AfterBlock in *. intros. destruct RA as [? [? ?]].
+  eapply (H0 _ (t1++(Addr (ei*4), s')::x)). 
+  rewrite app_cons, app_comm_cons in XP; apply exec_prog_split in XP as [_ [_ XP]].
+  pose proof (xp_splice _ _ _ _ H1 XP ltac:(now rewrite app_comm_cons, ostartof_niltail)).
+  simpl in H3. rewrite <-app_cons, (app_comm_cons x), app_assoc in H3. apply H3.
+  now apply Forall_forall.
+  rewrite (app_cons _ x), <-app_assoc.
+  apply Forall_app. split. easy. now inversion H2.
+Qed.
+Lemma afterblock_s:
+  forall P s bi len ei
+  (Q: InBlock (Z.of_N (bi+1) ) len (ei*4) ), 
+  AfterBlock P s (bi+1) len ei (fun t => fst t <> Addr (bi * 4)) ->
+  AfterBlock P s bi (len+1) ei (fun t => fst t <> Addr (bi*4)).
+Proof.
+  unfold AfterBlock. intros. eapply H. apply XP. easy.
+  apply Forall_app. split. apply Forall_app in IB as [? ?]. apply Forall_forall. rewrite Forall_forall in H0, T1. intros. unfold InBlockX, InBlock in *. destruct x, e.  apply H0 in H2 as ?. simpl in H3.
+  destruct H3. inversion H4. subst. apply T1 in H2. simpl in H2. enough (x <> bi). simpl. split. lia. now exists x. intro. subst. easy. 
+     apply H0 in H2. easy. constructor. easy.
+     easy.
+Qed.
+Lemma maintainsblock_s:
+  forall a b bi ei s, MaintainsBlock (a::b) bi ei s -> MaintainsBlock b (bi+1) ei s.
+Proof.
+  unfold MaintainsBlock. intros. destruct H. split. apply containsblock_cons in H. now rewrite N2Z.inj_add.
+  rewrite db_db' in *. unfold DuringBlock' in *. intros.
+      rewrite N2Z.inj_add. eapply containsblock_cons. eapply H0. apply XP. now rewrite Forall_forall. eapply Forall_impl. simpl. 
+      rewrite <-Nat.add_1_r. apply inblockx_ss.
+      apply IB. 
+Qed.
+
 Lemma afterblock_cond:
-  forall P b p s i l cond
+  forall P b s i l cond
   (B: arm_assemble_all_cond l cond = Some b)
   (I: i < 2^30 - 64)
   (L: (1 <= length l < 64)%nat)
-  (MB: MaintainsBlock p b i i s)
+  (MB: MaintainsBlock b i i s)
   (AB: match arm_assemble_all l with
-       | Some b' => forall s,
-           MaintainsBlock p b' (i + N.of_nat (length b - length b')) (i + N.of_nat (length b - length b')) s ->
-           AfterBlock P b' p s (i + N.of_nat (length b - length b')) (i + N.of_nat (length b - length b'))
+       | Some b' => forall s',
+           let i' := (i + N.of_nat (length b - length b')) in
+           (s' = s \/ Reachable i' s' i s i (length b)) ->
+           MaintainsBlock b' i' i' s' ->
+           AfterBlock P s' i' (length b') i' (fun t => fst t <> Addr (i*4))
        | _ => True
        end)
   (PA: forall s, P (Addr ((i + N.of_nat (length b))*4), s))
   (PS: forall s, P (Addr ((i + 1)*4), s)),
-    AfterBlock P b p s i i.
+    AfterBlock P s i (length b) i (fun _ => True).
 Proof.
   intros.
 
-  unfold arm_assemble_all_cond in B. destruct Z.ltb. 
+  unfold arm_assemble_all_cond in B. 
+   destruct Z.ltb.
+
+   eapply afterblock_nol.
+   intros.
     apply arm_assemble_all_first in B as [? [? [? [? ?]]]]. subst.
-    apply afterblock_cons. assumption. intros.
-    rewrite H1 in H0.
-    cbv[arm2il arm_b_il BranchWritePC arm_R] in H0. apply forget_cond in H0. remember (i*4). remember (scast _ _ _). step_stmt H0.
-    destruct N.modulo; destruct H0 as [H0 _]; step_stmt H0; destruct H0 as [[_ ?] _].
-
-      left. repeat split. assumption. simpl length in AB. rewrite H, Nat.sub_succ_l, Nat.sub_diag in AB. intro. apply AB. assumption. lia. easy.
-
+    eapply afterblock_step. destruct H. now subst. eapply mt. apply MB. apply H. easy. now rewrite Z.sub_diag, nth_error_O.
+    intros.
+    rewrite H2 in H1. assert (CP:=H1). mystep H1. mystep H1. destruct N.modulo; mystep H1; destruct H1 as [[? ?] _].
+      left. repeat split. assumption. simpl length in AB. rewrite H0, Nat.sub_succ_l, Nat.sub_diag in AB. intros ? ?R.
+      subst n. simpl. rewrite <-Nat.add_1_r. eapply afterblock_s. apply arm_assemble_all_len in H0. destruct x0. simpl in H0. lia. apply inblock_start. apply AB. 
+      right.
+      assert (exec_prog arm_prog ((Addr ((i+1)*4), reset_temps s' s'0)::(Addr (i*4), s')::nil)).
+      apply (exec_prog_step _ _ _ (exec_prog_none _ _)).
+      rewrite N.mul_add_distr_r.
+      eapply (CanStep _ (i*4) s' 4 _ _ _ None). destruct H. subst. destruct MB. specialize (c i inblock_start). rewrite Z.sub_diag, nth_error_O in c. apply c. 
+      eapply mt  in MB as [? ?]. specialize (H i inblock_start). rewrite Z.sub_diag, nth_error_O in H. apply H. easy. rewrite H2. subst. apply CP.
+      destruct H. exists nil. split. now subst. simpl. constructor. apply arm_assemble_all_len in H0. rewrite <-H0. unfold InBlockX, InBlock. split. lia. apply N.divide_factor_r. constructor. apply inblock_start. easy. destruct H as [? [? ?]]. pose proof (xp_splice _ (x2++(Addr (i*4), s)::nil) _ _ H H5 eq_refl). eexists.
+      split. simpl in *. rewrite app_comm_cons in H7. apply H7. constructor. unfold InBlockX, InBlock. split. apply arm_assemble_all_len in H0. lia. apply N.divide_factor_r. simpl. easy. eapply maintainsblock_s. apply H4. lia.
+       apply PS.
       assert (n ⊕ 8 ⊕ n0 .& 4294967292 = (i + N.of_nat (S(length l)))*4) as E.
       {
         subst.
         rewrite N.mul_add_distr_r, N.shiftl_mul_pow2. rewrite <-Z_nat_N, Z2Nat.inj_sub, Nat2Z.id, Nat2N.inj_sub, Z_nat_N by easy.
-        cbn. rewrite N.mul_sub_distr_r. unfold scast. epose proof (proj1 (toZ_nonneg _ _)). rewrite H0.
+        cbn. rewrite N.mul_sub_distr_r. unfold scast. pose proof (toZ_nonneg). edestruct H3. rewrite H4.
         rewrite (N.mod_small _ (2^26)), N2Z.inj_sub, N2Z.inj_mul, nat_N_Z by lia. cbn. unfold ofZ. rewrite Z2N.inj_mod by lia. replace (Z.to_N (_ - _)) with (N.of_nat (length l) * 4 - 4) by lia. rewrite <-N.Div0.add_mod.
         change 4294967296 with (2^32). rewrite N_land_mod_pow2_move by lia.
-        change (4294967292 mod 2 ^ 32) with (N.lnot (2 * (2 * 0 + 1) + 1) 32).
-        rewrite <- N.ldiff_land_low, 2 N.ldiff_odd_r, N.ldiff_0_r. lia. apply N.log2_lt_pow2. lia. lia. enough (N.of_nat (length l) * 4 - 4 < 2^ 25). rewrite N.mod_small by lia. apply H2. lia.
+        change (_ mod _) with (N.lnot (2 * (2 * 0 + 1) + 1) 32).
+        rewrite <- N.ldiff_land_low, 2 N.ldiff_odd_r, N.ldiff_0_r. lia. apply N.log2_lt_pow2. lia. lia. enough (N.of_nat (length l) * 4 - 4 < 2^ 25). rewrite N.mod_small by lia. apply H6. lia.
       }
-      simpl length in PA. apply arm_assemble_all_len in H.
-      right. right. left. repeat esplit. apply H0. rewrite E, H. apply PA.
+      simpl length in PA. apply arm_assemble_all_len in H0.
+      right. right. left. repeat esplit. apply H3. rewrite E, H0. apply PA.
       unfold InBlock. rewrite E. simpl length. lia.
 
-   rewrite B, Nat.sub_diag, N.add_0_r in AB. apply AB, MB.
+   eapply afterblock_nol. intros.
+   simpl in AB. rewrite B, Nat.sub_diag, N.add_0_r in AB. destruct H; apply AB. now left. now subst.
+   now right. eapply mt. apply MB. apply H.
 Qed.
 
 
 Lemma afterblock_fallthru:
-  forall P b b' p s bi, Forall (fun z => forall s c' s' x i a, exec_stmt armc s (arm2il i (arm_decode z)) c' s' x -> x <> Some (Addr a)) (b++[b']) ->
-  (forall a s, InBlock (Z.of_N bi) (length (b++[b'])) a -> P (Addr a, s)) ->
-  (MaintainsBlock p (b++[b']) bi bi s) ->
-  (forall s, P (Addr ((bi + N.of_nat (length (b++[b'])))*4), s)) -> AfterBlock P (b++[b']) p s bi bi.
+  forall n P b s bi T,
+  Forall (fun z => forall s c' s' x i a, exec_stmt armc s (arm2il i (arm_decode z)) c' s' x -> x <> Some (Addr a)) b ->
+  (forall a s, InBlock (Z.of_N bi) (length b) a -> P (Addr a, s)) ->
+  (0 < length b)%nat ->
+  (MaintainsBlock b bi (bi+(N.of_nat (length b) - 1 - n)) s) ->
+  (forall s, P (Addr ((bi + N.of_nat (length b))*4), s)) ->
+  AfterBlock P s bi (length b) (bi+(N.of_nat (length b) - 1 - n)) T.
 Proof.
-  induction b. - intros. simpl. apply afterblock_cons. simpl in H0. assumption. intros. destruct x. destruct e. inversion H. apply (H6 _ _ _ _ _ a) in H3. contradiction.
-  right. right. right. now exists i. right. left. repeat split. apply H2.
-  - simpl. intros. apply afterblock_cons. assumption. intros. destruct x. destruct e. inversion H. apply (H6 _ _ _ _ _ a0) in H3. contradiction.
-  right. right. right. now exists i. left. repeat split. intro. apply IHb. inversion H. assumption. intros. apply H0. unfold InBlock in *. split. lia. easy. assumption.
-  remember (length _). 
-  Search (_ + N.of_nat _). intros. 
-  rewrite <-(N2Nat.id 1), <-N.add_assoc, <- Nat2N.inj_add. apply H2. apply H0. split. rewrite length_app. simpl. lia. apply N.divide_factor_r.
+  induction n using N.peano_ind. intros. eapply afterblock_step. easy. lia.
+  replace_nth (length b - 1)%nat. apply nth_error_nth'. lia.
+  intros. rewrite Forall_nth in H. 
+  destruct x. destruct e.
+  eapply H in H4. easy. lia.
+  right. right. right. now exists i.
+  right. left. repeat split. lia. rewrite N.sub_0_r, <-N.add_assoc, N.sub_add by lia. apply H3.
+  intros. revert H2.
+  destruct (N.le_gt_cases (N.of_nat (length b) - 1) n). apply N.sub_0_le in H2. rewrite (proj2 (N.sub_0_le _ _)), <-H2 by lia. intro. now apply IHn.
+  intro.
+  eapply afterblock_step. easy. lia.
+  replace_nth (length b - 1 - N.to_nat (n + 1))%nat. apply nth_error_nth'. lia.
+  intros. assert (C:=H). rewrite Forall_nth in H.
+  destruct x. destruct e.
+  eapply H in H5. easy. lia.
+  right. right. right. now exists i.
+  destruct (Nat.eq_dec (length b) 1).
+  right. left. repeat split. lia. rewrite e, N.sub_diag, N.sub_0_l, N.add_0_r. now replace 1 with (N.of_nat (length b)) by lia.
+  left. repeat split. 
+  rewrite <-N.add_1_r, N.sub_add_distr, <-N.add_assoc, N.sub_add by lia. intros. now apply IHn.
+  apply H0. unfold InBlock. split. lia. apply N.divide_factor_r.
+  Unshelve. apply Z0. apply Z0.
 Qed.
 Lemma afterblock_fallthru':
-  forall P b p s bi, Forall (fun z => forall s c' s' x i a, exec_stmt armc s (arm2il i (arm_decode z)) c' s' x -> x <> Some (Addr a)) b -> 
+  forall P b s bi T,
+  Forall (fun z => forall s c' s' x i a, exec_stmt armc s (arm2il i (arm_decode z)) c' s' x -> x <> Some (Addr a)) b -> 
   (forall a s, InBlock (Z.of_N bi) (length b) a -> P (Addr a, s)) ->
-  (1 <= length b)%nat ->
-  (MaintainsBlock p b bi bi s) ->
-  (forall s, P (Addr ((bi + N.of_nat (length b))*4), s)) -> AfterBlock P b p s bi bi.
+  (0 < length b)%nat ->
+  (MaintainsBlock b bi bi s) ->
+  (forall s, P (Addr ((bi + N.of_nat (length b))*4), s)) -> AfterBlock P s bi (length b) bi T.
 Proof.
-  intros. destruct b. now simpl in H1. destruct (exists_last (ltac:(discriminate):z::b<>[])) as [? [? ?]]. rewrite e in *. now apply afterblock_fallthru.
+  intros. assert (bi = (bi+(N.of_nat (length b)-1-(N.of_nat (length b)-1)))) by lia.
+  rewrite H4 at 2. rewrite H4 in H2 at 2.
+  now apply afterblock_fallthru.
 Qed.
 
 
@@ -492,7 +765,7 @@ Proof.
   remember (_ - _ - _)%Z as offset. unfold Z2 in *.
   assert (src * 4 ⊕ 8 ⊕ scast 26 32 (Z.to_N (offset mod 16777216) << 2) .& 4294967292 = dest * 4).
   {
-    change 2 with (Z.to_N 2) at 2. rewrite <- Z2N_inj_shiftl, Z.shiftl_mul_pow2, <- Zmult_mod_distr_r by lia.
+change 2 with (Z.to_N 2) at 2. rewrite <- Z2N_inj_shiftl, Z.shiftl_mul_pow2, <- Zmult_mod_distr_r by lia.
     change (Z.to_N _) with (ofZ 26 (offset * 4)).
     unfold scast. rewrite toZ_ofZ by (unfold signed_range; cbn; lia). unfold ofZ.
     rewrite <- (N2Z.id ((_ + 8) mod _)), <- Z2N.inj_add, N2Z.inj_mod, <- (N2Z.id (_ ^ _)), <- Z2N.inj_mod, <- Zplus_mod by lia.
@@ -664,23 +937,320 @@ Local Ltac ft XS :=
 Local Ltac faft :=
   repeat constructor; solve [intros ?????? XS; ft XS] || assumption || idtac.
 
-Definition SafeAfterBlock i2i' pol ai i irm p s := AfterBlock (SafeDestX i2i' pol ai i (length irm)) irm p s (Z.to_N (i2i' i)) (Z.to_N (i2i' i)).
-Lemma SafeDest_rewrite_inst:
-  forall tc i2i' z pol i ti ai bi txt irm' table tc' p s1
-    (TC: True) (* table cache is consistent with memory *)
-    (AI: (0 <= ai < 2^30)%Z)
-    (TI: (0 <= ti < 2^30)%Z)
-    (I:  (0 <=  i < 2^30)%Z)
-    (BI: (0 <= bi < 2^30)%Z)
-    (AIB: ~ InBlock (i2i' i) (length irm') (Z.to_N ai * 4))
-    (I2I': (0 <= i2i' i < 2^30)%Z)
-    (I2I'': (i2i' (i + 1) = i2i' i + Z.of_nat (length irm'))%Z)
-    (RI: rewrite_inst tc i2i' z (pol i) i ti ai bi txt = Some (irm', table, tc'))
-    (MB: MaintainsBlock p irm' (Z.to_N (i2i' i)) (Z.to_N (i2i' i)) s1),
-
-    SafeAfterBlock i2i' pol ai i irm' p s1.
+Lemma exec_lsl:
+  forall reg s a c' s' x,
+  reg < 15 ->
+  exec_stmt arm7typctx s (arm2il a (LSL (Z.of_N reg) (Z.of_N reg) Z2)) c' s' x ->
+  reset_temps s s' = s[R_PC := a][arm_varid reg := (s (arm_varid reg) << 2) mod 2 ^ 32] /\ x = None.
+Proof.
+  intros. cbv[LSL arm2il arm_data_r_il arm_data_op_il arm_data_r_shiftc DecodeImmShift arm_data_il arm_cond_il arm_cond_exp arm_assign_R arm_R] in H0. simpl in H0. destruct N.eqb eqn:e; try lia.
+  rewrite N2Z.id in H0. unfold arm_varid. destruct_match_eqn; step_stmt H0; destruct H0; step_stmt H0; destruct H0 as [[? ?] ?]; lia || now rewrite H0.
+Qed.
+Definition LorB (R_E:N) := if R_E then LittleE else BigE.
+Lemma exec_ldr:
+  forall reg s a c' s' x,
+  reg < 15 ->
+  models armc s ->
+  exec_stmt armc s (arm2il a (LDR (Z.of_N reg) (Z.of_N reg) 0)) c' s' x ->
+  reset_temps s s' = s[R_PC := a][arm_varid reg := getmem 32 (LorB (s R_E)) 4 (s V_MEM32) (s (arm_varid reg))] /\ x = None.
 Proof.
   intros.
+  cbv[LDR arm2il arm_ls_i_il arm_ls_op_il arm_ls_il arm_cond_il arm_cond_exp arm_assign_R arm_MemU] in H1.
+  simpl in H1. rewrite !N2Z.id in H1. destruct N.eqb eqn:e; try lia.
+  specialize (H0 (arm_varid reg) 32).
+  unfold arm_varid. destruct_match_eqn; try lia; step_stmt H1; destruct H1; step_stmt H1; simpl in H1; destruct H1 as [[? ?] _];
+  rewrite H1, N.add_0_r, N.mod_small by (now apply H0); destruct (s R_E); now subst.
+Qed.
+Lemma exec_bx:
+  forall reg s a c' s' x,
+  reg < 15 ->
+  (4 | s (arm_varid reg)) ->
+  exec_stmt armc s (arm2il a (ARM_BX 14 (Z.of_N reg))) c' s' x ->
+  x = Some (Addr (s (arm_varid reg))).
+Proof.
+  intros.
+  cbv[arm2il arm_bx_il arm_cond_il arm_cond_exp BXWritePC arm_R] in H1. simpl in H1.
+  rewrite N2Z.id in H1.
+  change 4 with (2^2) in H0. inversion H0.
+  unfold arm_varid. destruct_match_eqn; try lia; simpl arm_varid in *;
+  step_stmt H1; destruct H1; step_stmt H1;
+  rewrite N.shiftr_0_r, N.Div0.mul_mod, N.mul_0_r, N.Div0.mod_0_l in H1; destruct H1;
+  step_stmt H1; rewrite N.shiftr_div_pow2, <-N.testbit_spec', N.mul_pow2_bits_low in H1 by lia; destruct H1; step_stmt H1; destruct H1 as [[_ ?] _]; now rewrite H1, H2.
+Qed.
+Local Lemma typeof_arm_varid:
+  forall n, arm7typctx (arm_varid n) = Some 32.
+Proof.
+  intros. unfold arm_varid. now destruct_match.
+Qed.
+Lemma exec_str :
+  forall rt rn s s' a c' x offset
+    (XS: exec_stmt armc s (arm2il a (STR (Z.of_N rt) (Z.of_N rn) (-(Z.of_N offset)))) c' s' x)
+    (RT: rt < 15)
+    (RN: rn < 15)
+    (O: 0 < offset)
+    (M: models armc s),
+    getmem 32 (LorB (s R_E)) 4 (s' V_MEM32) (s (arm_varid rn) ⊖ offset) = s (arm_varid rt).
+Proof.
+  (* intros. cbv[STR arm2il arm_ls_i_il arm_ls_op_il arm_ls_il Z1 Z14 arm_assign_MemU arm_cond_il arm_cond_exp ] in XS. *)
+  (* replace (- _ <? _)%Z with true in XS by lia. *)
+  (* simpl Z.to_N in XS. cbv[N.eqb orb Pos.eqb] in XS. simpl in XS. *)
+  (* cbv[arm_R] in XS. *)
+  (* rewrite !N2Z.id in XS. *)
+  (* replace (Z.to_N _) with (offset) in XS by lia. *)
+  (* replace (rn =? 15) with false in XS by lia. replace (rt0 =? 15) with false in XS by lia.  *)
+  (* specialize (M (arm_varid rt0) _ (typeof_arm_varid _)). unfold arm_varid in *. destruct_match_eqn; try lia; *)
+  (* step_stmt XS; destruct XS as [XS _]; step_stmt XS; destruct XS as [XS _]; destruct (s R_E); step_stmt XS; destruct XS as [[? ?] [? _]]; *)
+  (* rewrite <-(reset_temps_not_temp _ s), H, update_updated by discriminate; now rewrite getmem_setmem, N.mod_small by lia. *)
+Admitted.
+Lemma reset_temps_update_r:
+  forall s s' n v v', reset_temps s (s'[R_PC := v][arm_varid n := v']) = (reset_temps s s')[R_PC := v][arm_varid n := v'].
+Proof.
+  intros. unfold reset_temps, arm_varid. now rewrite reset_vars_fchoose, !fchoose_update_distr, !fchoose_update_l by now destruct_match_eqn.
+Qed.
+Lemma arm_varid_not_pc:
+  forall n, n < 15 -> arm_varid n <> R_PC.
+Proof.
+  intros. unfold arm_varid. destruct_match_eqn; discriminate || lia.
+Qed.
+Lemma after_arm_table_lookup:
+  forall P ti sl sr reg s bi ei b prefix tail T
+  (B: arm_assemble_all (prefix++arm_table_lookup (Z.of_N ti) sl (Z.of_N sr) (Z.of_N reg)++tail) = Some b)
+  (MB: MaintainsBlock b bi (bi + N.of_nat (length prefix)) s)
+  (REG: reg < 15)
+  (SR: sr < 32)
+  (EI: ei = bi + N.of_nat (length prefix))
+  (M: models armc s)
+  (* block does not wrap around *)
+  (I: bi + N.of_nat (length b) < 2 ^ 30)
+  (* block continues after arm_table_lookup *)
+  (TL: (0 < length tail)%nat)
+  (* table does not wrap around *)
+  (TB: ti + 2 ^ (32 - sr) < 2 ^ 30)
+  (* P holds while still in the block *)
+  (IB: (forall xs, InBlockX bi (length b) xs -> P xs))
+  (PC: forall s' n,
+    MaintainsBlock b bi (ei+7) s' ->
+    Reachable (ei+7) s' ei s bi (length b) ->
+    (* the store after arm_table_lookup finishes executing has reg set to Mem[n*4] (endianness depends on R_E) *)
+    reset_temps s s' = s[R_PC := (bi + N.of_nat (length prefix) + 6) * 4][arm_varid reg := getmem 32 (LorB (s R_E)) 4 (s V_MEM32) (n*4)] ->
+    (* n is an index of the table *)
+    ti <= n < ti + 2 ^ (32 - sr) ->
+    AfterBlock P s' bi (length b) (ei+7) T),
+  AfterBlock P s bi (length b) ei T.
+Proof.
+  intros. unfold arm_table_lookup in B. cbn [app] in B. move B after PC.
+  pose proof (arm_varid_not_pc reg REG) as NOTPC. pose proof (not_eq_sym NOTPC) as NOTPC'. move NOTPC' after REG. move NOTPC after REG.
+
+  assert (B':=B).
+  apply arm_assemble_all_app in B as [b_pre [b_tail [? [BPRE B]]]]; subst; rename b_tail into b.
+  apply arm_assemble_all_len in BPRE. rewrite length_app in I.
+  (* UBFX *)
+  apply arm_assemble_all_first in B as [z_ubfx [b_tail [B [B_B' DECODE]]]]; subst; rename b_tail into b.
+  eapply afterblock_step; [assumption|lia|..].
+  replace_nth (length prefix). now rewrite BPRE, nth_error_app2, Nat.sub_diag, nth_error_O by easy. 
+
+  intros ??? XS. left. eapply (pres_frame_exec_stmt M M) in XS as M0; [|apply welltyped_arm2il; lia]. rewrite DECODE in XS; clear DECODE.
+  apply UBFX_bound in XS as [reg_val [? [REGBOUND EXIT]]];[|lia ..]; subst; clear c'.
+  rewrite reset_temps_update_r, reset_temps_id.
+  repeat split; [|shelve]. clear MB; intros MB RA.
+
+  (* LSL *)
+  apply arm_assemble_all_first in B as [z_lsl [b_tail [B [B_B' DECODE]]]]; subst; rename b_tail into b.
+  eapply afterblock_step; [assumption|lia|..].
+  replace_nth (length prefix + 1)%nat. rewrite nth_error_app2 by lia. now replace_nth 1%nat.
+  simpl in I.
+  intros ??? XS. left. eapply (pres_frame_exec_stmt M0 M0) in XS as M1; [|apply welltyped_arm2il; lia]. rewrite DECODE in XS; clear DECODE.
+  apply exec_lsl in XS as [S' EXIT]; [|lia]; subst; clear c'.
+  rewrite N2Z.id, !update_cancel2, update_updated, reset_temps_update_l, N.shiftl_mul_pow2 in S' by assumption.
+  repeat split; [|shelve].
+  rewrite <-N.add_assoc, N2Z.id, reset_temps_update_l.
+  (* replace (z_lsl::b) with ((z_lsl::nil)++b) by easy. change (1+1) with (1+N.of_nat (length (z_lsl::nil))). *)
+  rewrite N.add_assoc. simpl.
+  clear MB; intros MB ?. rewrite N2Z.id in RA. r.
+
+  
+  (* arm_add *)
+  unfold Z4 in B. rewrite <-app_cons, <-(Z2N.id (_ * _)) in B by lia. simpl.
+  eapply after_arm_add.
+    easy.
+    now apply reset_temps_models.
+    shelve.
+    rewrite cons_cons, <-app_cons, app_assoc, <-(Z2N.id Z4), <-N2Z.inj_mul in B' by (unfold Z4; lia). apply B'.
+    simpl. lia.
+    lia.
+    rewrite length_app. simpl. apply arm_assemble_all_len in B. simpl in B. lia.
+    assumption.
+  clear MB; intros s'' MB ? M2 S''. r.
+  rewrite reset_temps_overwrite_l, S', N2Z.id, !update_cancel2, update_updated in S'' by assumption.
+
+  (* LDR *)
+  apply arm_assemble_all_app in B as [b_add [b_tail [B_add_tail [BADD B]]]]; subst; rename b_tail into b.
+  apply arm_assemble_all_len in BADD. simpl in BADD.
+  apply arm_assemble_all_first in B as [z_ldr [b_tail [B [B_B' DECODE]]]]; subst; rename b_tail into b.
+  apply afterblock_step with (z:=z_ldr); [assumption|lia|..].
+  replace_nth (length prefix + 6)%nat. rewrite nth_error_app2 by lia. replace_nth 6%nat. rewrite 2nth_error_S. simpl tl. rewrite nth_error_app2 by lia. now rewrite <-BADD.
+  intros c' s''' x XS. eapply (pres_frame_exec_stmt M2 M2) in XS as M3; [|apply welltyped_arm2il; rewrite BPRE; rewrite length_app in I; try lia]. rewrite DECODE in XS; clear DECODE.
+  apply exec_ldr in XS as [S''' EXIT]; [|lia|assumption]; subst; clear c'.
+
+  rewrite <-(reset_temps_not_temp R_E s), <-(reset_temps_not_temp V_MEM32 s), <-(reset_temps_not_temp (arm_varid reg) s) in S''' by (try rewrite typeof_arm_varid; discriminate).
+  rewrite S'', update_updated, !update_frame in S''' by (unfold arm_varid; destruct_match_eqn; discriminate).
+  rewrite <-(reset_temps_revert s), reset_temps_update_l, reset_temps_update_r, S'', !reset_temps_update_r, !update_cancel2 in S''' by assumption.
+  rewrite N.Div0.add_mod_idemp_l, (N.mul_comm _ ti), <-N.mul_add_distr_r in S'''.
+  left. repeat split; [|shelve].
+  rewrite <-3N.add_assoc. simpl.
+  clear MB; intros MB ?. r.
+
+  unfold Z4 in *.
+  apply (PC _ (reg_val+ti)). assumption. assumption. rewrite S''', reset_temps_update_r, reset_temps_revert, N.mod_small, <-2N.add_assoc by lia.
+  reflexivity.
+  lia.
+
+  Unshelve.
+  3: rewrite length_app; simpl; lia.
+  all: apply arm_assemble_all_len in B; simpl in B; apply IB.
+  all: unfold InBlockX, InBlock; simpl; split; [|apply N.divide_factor_r].
+  all: rewrite length_app; simpl; try rewrite length_app; simpl; lia.
+Qed.
+
+Definition SafeAfterBlock i2i' pol ai i len s := AfterBlock (SafeDestX i2i' pol ai i len) s (Z.to_N (i2i' i)) len (Z.to_N (i2i' i)) (fun _ => True).
+Lemma find_sr_bound:
+  forall dis dis' sl sr a, find_sr dis dis' sl sr = Some a -> (0 <= a <= sr)%Z.
+Proof.
+  intros ?????. apply find_sr_ind.
+    easy.
+    intros. inversion H. lia.
+    intros. unfold Z1 in *. apply H in H0. lia.
+Qed.
+Lemma find_hash_bound:
+  forall dis dis' sl a b, find_hash dis dis' sl = Some (a, b) -> (0 <= b < 32)%Z.
+Proof.
+  intros ?????. apply find_hash_ind.
+    easy.
+    intros. inversion H. subst. unfold Z31 in e0. apply find_sr_bound in e0. lia.
+    intros. now apply H.
+Qed.
+Lemma map2list_len:
+  forall m n, length (_map2list m n) = n.
+Proof.
+  induction n. easy. simpl. now rewrite IHn.
+Qed.
+Lemma make_jump_table_len:
+  forall dis dis' ai sl sr n, length (make_jump_table dis dis' ai sl sr n) = Z.to_nat n.
+Proof.
+  intros. unfold make_jump_table. rewrite length_rev, map2list_fix. now rewrite map2list_len.
+Qed.
+Definition SafeTableCache i2i' pol ai tbi (flattened_tables: list Z) (tc: TableCache) :=
+  forall si ti sl sr
+    (TC: tc (pol si) = Some (ti, sl, sr)),
+    exists table,
+      extract_table sr tbi ti flattened_tables = Some table /\
+      SafeTable i2i' pol ai si table /\
+      ((0 <= sr < 32)%Z /\ (0 <= sl)%Z /\ (0 <= ti) /\ (ti + 2 ^ (32 - sr) < 2 ^ 30))%Z.
+
+Lemma table_size_correctness:
+  forall sr tbi ti flattened_tables t
+    (T: extract_table sr tbi ti flattened_tables = Some t),
+    length t = compute_table_size sr.
+Proof.
+  intros. unfold extract_table in T. destruct_match_in T; try discriminate.
+  inversion T. rewrite length_firstn, length_skipn. lia.
+Qed.
+Lemma afterblock_timpl:
+  forall P s bi len ei T T', (forall t, T t -> T' t) -> AfterBlock P s bi len ei T' -> AfterBlock P s bi len ei T.
+Proof.
+  unfold AfterBlock. intros. eapply H0. apply XP. eapply Forall_impl. apply H. easy. easy.
+Qed.
+Lemma afterblock_sq:
+  forall P s bi len ei
+  (Q: InBlock (Z.of_N (bi+1) ) len (ei*4) ), 
+  AfterBlock P s (bi+1) len ei (fun t => fst t <> Addr (bi * 4)) ->
+    AfterBlock P s bi (S len) ei (fun t => fst t <> Addr (bi*4)).
+Proof.
+  unfold AfterBlock. intros. eapply H. apply XP. easy.
+  apply Forall_app. split. apply Forall_app in IB as [? ?]. apply Forall_forall. rewrite Forall_forall in H0, T1. intros. unfold InBlockX, InBlock in *. destruct x, e.  apply H0 in H2 as ?. simpl in H3.
+  destruct H3. inversion H4. subst. apply T1 in H2. simpl in H2. enough (x <> bi). simpl. split. lia. now exists x. intro. subst. easy. 
+     apply H0 in H2. easy. constructor. easy.
+     easy.
+Qed.
+Lemma reachablegrow {i2 s2 i1 s1 bi len bi' len'}:
+forall
+    (RA: Reachable i2 s2 i1 s1 bi len)
+    (START: bi' <= bi)
+    (END: bi+N.of_nat len <= bi'+N.of_nat len'),
+    Reachable i2 s2 i1 s1 bi' len'.
+Proof.
+  intros. destruct RA as [? [?]]. eexists. split. apply H. eapply Forall_impl. shelve. apply H0. Unshelve.
+  unfold InBlockX, InBlock. intros. destruct fst. split. lia. easy. easy.
+Qed.
+  
+
+Lemma exec_ldrpc:
+  forall s a c' s' x
+    (XS: exec_stmt armc s (arm2il a (LDR PC SP Z_8)) c' s' x)
+    (D: (4 | getmem 32 (LorB (s R_E)) 4 (s V_MEM32) (s R_SP ⊖ 8)))
+    (S: (4 | s R_SP)),
+    x = Some (Addr (getmem 32 (LorB (s R_E)) 4 (s V_MEM32) (s R_SP ⊖ 8))).
+Proof.
+  intros. cbv[LDR arm2il arm_ls_i_il arm_ls_op_il arm_ls_il arm_cond_il Z1] in XS.
+  simpl Z.to_N in XS. cbv[N.eqb orb Pos.eqb arm_cond_exp BXWritePC arm_R arm_varid] in XS . simpl in XS.
+  step_stmt XS. destruct XS as [XS _]. step_stmt XS. replace (_ =? _) with true in XS. simpl in XS. destruct XS as [XS _].
+  step_stmt XS. replace (_ mod _) with 0 in XS. destruct XS as [XS _]. step_stmt XS. replace (_ =? 1) with false in XS. destruct XS as [XS _].
+  step_stmt XS. destruct XS as [[? ?] _]. destruct (s R_E). now subst. now subst. rewrite <-N.bit0_eqb, N.shiftr_spec'. 
+  destruct (s R_E);  destruct D; simpl in H; rewrite H; change 4 with (2^2); now rewrite N.mul_pow2_bits_low. 
+  destruct (s R_E);  destruct D; simpl in H; rewrite H; simpl; lia.
+  destruct S. rewrite H. unfold msub. simpl N.sub. change 4294967288 with (1073741822*4). rewrite <-N.mul_add_distr_r.
+  rewrite N_land_mod_pow2_move.
+  change (_ mod _) with (N.ones 2).
+  rewrite N.land_ones. lia.
+Qed.
+Lemma SafeDest_rewrite_inst:
+  forall tc i2i' z pol i ti ai bi txt irm' table tc' s1 tbi flattened_tables
+    (RI: rewrite_inst tc i2i' z (pol i) i ti ai bi txt = Some (irm', table, tc'))
+    (TC: SafeTableCache i2i' pol ai tbi flattened_tables tc) 
+    (AI: (0 <= ai < 2^30)%Z)
+    (TI: (0 <= ti)%Z)
+    (TI': (ti + Z.of_nat (length table) < 2^30)%Z)
+    (I:  (0 <=  i < 2^30)%Z)
+    (BI: (0 <= bi < 2^30)%Z)
+    (M: models armc s1)
+    (MB: MaintainsBlock irm' (Z.to_N (i2i' i)) (Z.to_N (i2i' i)) s1)
+    (* abort index is not in this block *)
+    (AIB: ~ InBlock (i2i' i) (length irm') (Z.to_N ai * 4))
+    (* new indices are in range *)
+    (I2I: forall i, (0 <= i2i' i < 2^30-64)%Z)
+    (* the block of the next instruction is placed right after the end of this block *)
+    (I2I'': (i2i' (i + 1) = i2i' i + Z.of_nat (length irm'))%Z)
+    (* no new indices start inside of this block *)
+    (I2I''': forall j, (i2i' j <= i2i' i \/ i2i' i + Z.of_nat (length irm') <= i2i' j)%Z)
+    (* new table is in memory *)
+    (TIM: forall n,
+      Z.to_N ti <= n < Z.to_N ti + N.of_nat (length table) ->
+      In (Z.of_N (getmem 32 (LorB (s1 R_E)) 4 (s1 V_MEM32) (n*4))) table
+    )
+    (* everything tc returns is in memory *)
+    (TCIM: forall si ti sl sr n t,
+      tc si = Some (ti, sl, sr) ->
+      extract_table sr tbi ti flattened_tables = Some t ->
+      Z.to_N ti <= n < Z.to_N ti + N.of_nat (length t) ->
+      In (Z.of_N (getmem 32 (LorB (s1 R_E)) 4 (s1 V_MEM32) (n*4))) t
+    )
+    (* new table is not writable *)
+    (NWT: DuringBlock (fun xs => forall n e,
+      Z.to_N ti <= n < Z.to_N ti + N.of_nat (length table) ->
+      getmem 32 e 4 (snd xs V_MEM32) (n*4) = getmem 32 e 4 (s1 V_MEM32) (n*4)) s1 (Z.to_N (i2i' i)) (length irm') (Z.to_N (i2i' i)) (fun _ => True)
+    )
+    (* nothing tc returns is writable *)
+    (NWTC: forall si ti sl sr t,
+      tc si = Some (ti, sl, sr) ->
+      extract_table sr tbi ti flattened_tables = Some t ->
+      DuringBlock (fun xs => forall n e, Z.to_N ti <= n < Z.to_N ti + N.of_nat (length t) -> getmem 32 e 4 (snd xs V_MEM32) (n*4) = getmem 32 e 4 (s1 V_MEM32) (n*4)) s1 (Z.to_N (i2i' i)) (length irm') (Z.to_N (i2i' i)) (fun _ => True))
+    (* endian flag does not change *)
+    (E: DuringBlock (fun xs => snd xs R_E = s1 R_E) s1 (Z.to_N (i2i' i)) (length irm') (Z.to_N (i2i' i)) (fun _ => True)),
+
+    SafeAfterBlock i2i' pol ai i (length irm') s1.
+Proof.
+  intros. apply SafeTable_rewrite_inst in RI as ST.
+  specialize (I2I i) as I2I'.
 
   assert (
     forall l cond, arm_assemble_all_cond l cond = Some irm' ->
@@ -688,40 +1258,211 @@ Proof.
       In (Z.add i 1) (pol i) ->
       match arm_assemble_all l with
       | Some b' => forall s,
-        MaintainsBlock p b'
-          (Z.to_N (i2i' i) + N.of_nat (length irm' - length b'))
-          (Z.to_N (i2i' i) + N.of_nat (length irm' - length b')) s ->
-        AfterBlock (SafeDestX i2i' pol ai i (length irm')) b' p s
-          (Z.to_N (i2i' i) + N.of_nat (length irm' - length b'))
-          (Z.to_N (i2i' i) + N.of_nat (length irm' - length b'))
+          let i' := (Z.to_N (i2i' i) + N.of_nat (length irm' - length b')) in
+        (s = s1 \/ Reachable i' s (Z.to_N (i2i' i)) s1 (Z.to_N (i2i' i)) (length irm')) ->
+        MaintainsBlock b' i' i' s ->
+        AfterBlock (SafeDestX i2i' pol ai i (length irm')) s i' (length b') i' (fun xs => fst xs <> Addr (Z.to_N (i2i' i) * 4))
       | None => True
       end ->
-    SafeAfterBlock i2i' pol ai i irm' p s1
+    SafeAfterBlock i2i' pol ai i (length irm') s1
   ) as C. {
-    intros. eapply afterblock_cond. apply H. admit. assumption. assumption. assumption. 
-      intros. unfold SafeDestX, SafeDest. simpl. left. right. exists (i+1)%Z. split. unfold i2a', to_a. lia. assumption.
+    intros. eapply afterblock_cond. apply H. lia. assumption. assumption. assumption.
+      intros. unfold SafeDestX, SafeDest. simpl. left. right. exists (i+1)%Z. split. lia. assumption.
       intros. unfold SafeDestX, SafeDest. simpl. 
-      destruct (Nat.eq_dec (length irm') 1). left. right. exists(i+1)%Z. split. unfold i2a', to_a. lia. assumption.
+      destruct (Nat.eq_dec (length irm') 1). left. right. exists(i+1)%Z. split. lia. assumption.
       right. unfold InBlock. split. split. lia.
       apply arm_assemble_all_cond_len in H.
       lia. apply N.divide_factor_r.
+  }
+
+  assert (forall irm cond
+  (RWT: rewrite_w_table irm tc (pol i) i2i' cond i ti ai = Some (irm', table, tc'))
+  (SI: forall ti sl sr
+    (IRM: irm cond i ti sl sr = Some irm')
+    (TI: (0 <= ti)%Z)
+    (TI': Z.to_N ti + 2 ^ (32 - Z.to_N sr) < 2 ^ 30)
+    (SR: (0 <= sr < 32)%Z)
+    (N: forall n s i',
+      Z.to_N ti <= n < Z.to_N ti + 2 ^ (32 - Z.to_N sr) ->
+      s = s1 \/
+      Reachable i' s (Z.to_N (i2i' i)) s1 (Z.to_N (i2i' i)) (length irm') ->
+      SafeEntry i2i' pol ai i (Z.of_N (getmem 32 (LorB (s R_E)) 4 (s V_MEM32) (n*4)))
+    ),
+    SafeAfterBlock i2i' pol ai i (length irm') s1),
+  SafeAfterBlock i2i' pol ai i (length irm') s1) as RWT. {
+    intros. unfold rewrite_w_table in RWT. destruct_match_in RWT; try discriminate.
+    inversion RWT. subst. apply SI in e2. easy. apply TC in e. now destruct e. apply TC in e. destruct e.
+    apply N2Z.inj_lt. rewrite N2Z.inj_add, N2Z.inj_pow, N2Z.inj_sub, !Z2N.id by lia. lia.
+    apply TC in e. now destruct e. intros.
+    assert (ee:=e).
+    apply TC in e as [table [XT ST']]. unfold SafeTable in ST'. rewrite Forall_forall in ST'.
+    specialize (NWTC _ _ _ _ _ ee XT).
+    apply table_size_correctness in XT as TS. unfold compute_table_size in TS.
+    eapply TCIM in ee. apply ST' in ee. destruct H0. rewrite e. apply ee. 
+    apply (reachableduring r) in E. simpl in E. rewrite E. 
+    eapply (reachableduring r) in NWTC. simpl in NWTC. rewrite NWTC. easy. rewrite TS.
+    rewrite Z_nat_N, Z2N.inj_pow, Z2N.inj_sub. easy. easy. lia. lia.
+    easy. rewrite TS, Z_nat_N, Z2N.inj_pow, Z2N.inj_sub by lia. easy.
+    remember (make_jump_table _ _ _ _ _ _).
+    apply find_hash_bound in e0. 
+    unfold Z32 in *. rewrite Z.shiftl_mul_pow2, Z.mul_1_l in Heql0 by lia.
+    inversion RWT. subst. apply SI in e2. easy. easy. apply N2Z.inj_lt. rewrite N2Z.inj_add, N2Z.inj_pow, N2Z.inj_sub, !Z2N.id by lia. 
+    rewrite make_jump_table_len, Z2Nat.id in TI' by lia. lia.
+    lia. intros. rewrite make_jump_table_len, Z_nat_N, Z2N.inj_pow, Z2N.inj_sub in TIM by lia. 
+    apply TIM in H as IN. unfold SafeTable in ST. rewrite Forall_forall in ST. apply ST in IN. destruct H0. rewrite H0. easy.
+    apply (reachableduring H0) in NWT. rewrite NWT. apply (reachableduring H0) in E. simpl in E. rewrite E. easy. 
+    rewrite make_jump_table_len. rewrite Z_nat_N, Z2N.inj_pow, Z2N.inj_sub by lia. apply H.
+  }
+
+  assert (forall j
+    (SE: SafeEntry i2i' pol ai i (Z.of_N j)),
+    ~InBlock (i2i' i) (length irm') j \/ j = Z.to_N (i2i' i * 4)%Z) as SENIB.
+  {
+    intros. destruct SE.
+      left. intro. apply AIB.
+        rewrite <-(Z2N.id (ai*4)) in H by lia. apply N2Z.inj in H. rewrite Z2N.inj_mul in H by lia. simpl in H. now rewrite H.
+      destruct H as [? [? ?]]. edestruct inblock_dec. shelve.
+        left. apply n.
+        Unshelve. right. unfold InBlock in *. specialize (I2I''' x). lia.
+  }
+  assert (forall j
+    (SE: SafeEntry i2i' pol ai i (Z.of_N j)),
+    (4 | j)) as SE4. {
+    intros. destruct SE.
+      rewrite <-(Z2N.id (ai*4)) in H by lia. apply N2Z.inj in H. rewrite <-H, Z2N.inj_mul by lia. apply N.divide_factor_r.
+      destruct H as [? [? ?]]. rewrite <-(Z2N.id (_*_)) in x0 by lia. apply N2Z.inj in x0.
+        specialize (I2I x). rewrite <-x0, Z2N.inj_mul by lia. apply N.divide_factor_r.
+  }
+
+    Ltac mylia := unfold SafeDestX, SafeDest, InBlockX, InBlock in *; 
+      repeat match goal with
+             | H := _ |- _ => simpl in H; subst H
+             end;
+             try rewrite length_app in *; simpl length in *;
+      repeat match goal with
+             | H: arm_assemble_all_cond _ _ = Some _ |- _ => apply arm_assemble_all_cond_len in H; simpl in H
+             | H: arm_assemble_all _ = Some _ |- _ => apply arm_assemble_all_len in H; simpl in H; try rewrite <-H in *
+             | H: _ = Some (?irm, _, _), H1: _ = Some ?irm |- _ => try apply arm_assemble_all_cond_len in H1; simpl in H1
+             end; 
+             match goal with |- _ /\ (4 | _) => split; [try lia|try apply N.divide_factor_r] | |- _ => try lia end.
+
+  assert (forall reg cond
+    (RB: rewrite_bx reg tc (pol i) i2i' cond i ti ai = Some (irm', table, tc'))
+    (R: (0 <= reg < 15)%Z)
+    (PA: In (Z.add i 1) (pol i)),
+    SafeAfterBlock i2i' pol ai i (length irm') s1
+  ) as RBX. {
+    intros. eapply RWT.
+    apply RB. intros. eapply C. apply IRM. simpl. lia. assumption.
+    destruct arm_assemble_all eqn:B; auto. intros.
+    eapply after_arm_table_lookup with (prefix:=nil). 
+    rewrite <-(Z2N.id ti0), <-(Z2N.id sr), <-(Z2N.id reg) in B by lia. rewrite app_nil_l. apply B.
+    now rewrite N.add_0_r. lia. lia. simpl; lia.
+    destruct H. now rewrite H. destruct H as [? [? ?]]. apply (preservation_exec_prog arm_prog welltyped_arm_prog _ _ _ _ _ H ltac:(now rewrite startof_niltail) M).
+    mylia. 
+    simpl. lia. lia. 
+    intros. destruct xs, e. right. unfold i' in H1. cbn in H1. unfold InBlock in *. split. apply arm_assemble_all_cond_len in IRM. simpl in IRM. apply arm_assemble_all_len in B. simpl in B. inversion RB. subst. lia. now destruct H1. easy.
+
+    intros ??? RA ??. 
+
+  apply arm_assemble_all_app in B as [b_add [b_tail [B_add_tail [BADD B]]]]; subst; rename b_tail into b.
+  apply arm_assemble_all_len in BADD. simpl in BADD.
+  apply arm_assemble_all_first in B as [z_bx [b_tail [B [B_B' DECODE]]]]; subst; rename b_tail into b.
+    apply afterblock_step with (z:=z_bx).
+    easy. lia.
+    replace_nth 7%nat. rewrite nth_error_app2. now rewrite <-BADD. lia.
+    intros.
+  rewrite DECODE in H4. rewrite <-(Z2N.id reg) in H4 by lia. 
+  apply exec_bx in H4.
+  rewrite <-(reset_temps_not_temp _ s), H2, update_updated in H4 by (rewrite typeof_arm_varid; discriminate).
+  right. right. left. eexists. repeat split. apply H4. left. eapply (N _ _ _ H3 H). 
+  destruct (SENIB _ (N _ _ _ H3 H)). left. intro. apply H5. mylia. easy. right. now rewrite H5, Z2N.inj_mul by lia.
+  lia. rewrite <-(rt s), H2, update_updated. apply (SE4 _ (N _ _ _ H3 H)).
+  }
+
+
+  assert (forall sanitized_inst reg cond
+  (RPC: rewrite_pc sanitized_inst reg tc (pol i) i2i' cond i ti ai = Some (irm', table, tc'))
+  (FT: forall s c' s' x i a, exec_stmt armc s (arm2il i sanitized_inst) c' s' x  -> x <> Some (Addr a))
+  (R: (0 <= reg < 15)%Z)
+  (IN: In (Z.add i 1) (pol i)),
+  SafeAfterBlock i2i' pol ai i (length irm') s1) as RP. {
+    intros. eapply RWT. apply RPC. intros. eapply C. apply IRM. simpl. lia. assumption.
+    destruct arm_assemble_all eqn:B; auto. clear MB. intros s i' RA MB. assert (B':=B).
+
+    apply arm_assemble_all_first in B as [z_str [b_tail [B [B_B' DECODE]]]]; subst; rename b_tail into b.
+    eapply afterblock_step. assumption. lia. now replace_nth O. intros ??? XS. rewrite DECODE in XS; clear DECODE.
+    eapply arm_ls_i_fallthru in XS; [|right;discriminate].
+    left. repeat split. assumption. rename MB into MM. rename RA into RR. intros MB RA.
+
+    apply arm_assemble_all_first in B as [z_movw [b_tail [B [B_B' DECODE]]]]; subst; rename b_tail into b.
+    eapply afterblock_step. assumption. lia. now replace_nth 1%nat. intros ??? XS. rewrite DECODE in XS;clear DECODE.
+    apply arm_movwt_fallthru in XS.
+    left. repeat split. assumption. rewrite reset_temps_overwrite_l. clear MB; intros MB ?. r.
+
+    apply arm_assemble_all_first in B as [z_movt [b_tail [B [B_B' DECODE]]]]; subst; rename b_tail into b.
+    eapply afterblock_step. assumption. lia. now replace_nth 2%nat. intros ??? XS. rewrite DECODE in XS;clear DECODE.
+    apply arm_movwt_fallthru in XS.
+    left. repeat split. assumption. rewrite reset_temps_overwrite_l. clear MB; intros MB ?. r.
+
+    apply arm_assemble_all_first in B as [z_sanitized [b_tail [B [B_B' DECODE]]]]; subst; rename b_tail into b.
+    eapply afterblock_step. assumption. lia. now replace_nth 3%nat. intros ??? XS. destruct x.
+      destruct e. now eapply FT in XS. right. right. right. now exists i0.
+    left. repeat split. rewrite reset_temps_overwrite_l. clear MB; intros MB ?. r.
+
+    eapply after_arm_table_lookup. 
+    rewrite <-(Z2N.id ti0), <-(Z2N.id sr), <-(Z2N.id reg) in B' by lia. apply B'.
+      now rewrite <-3N.add_assoc in MB.
+      lia.
+      lia.
+      simpl. lia.
+      shelve.
+      mylia.
+      simpl. lia.
+      lia.
+      intros. simpl. destruct xs, e. simpl in H. right. split. mylia. simpl in H. lia. now inversion H. easy.
+      clear MB; intros ?? MB ? AAA NB. simpl in AAA. rewrite reset_temps_overwrite_l in AAA.
+
+  apply arm_assemble_all_app in B as [b_add [b_tail [B_add_tail [BADD B]]]]; subst; rename b_tail into b.
+  apply arm_assemble_all_len in BADD. simpl in BADD.
+  apply arm_assemble_all_first in B as [z_str' [b_tail [B [B_B' DECODE]]]]; subst; rename b_tail into b.
+  eapply afterblock_step. simpl in MB. now rewrite <-!N.add_assoc in *. lia. replace_nth 11%nat. rewrite !nth_error_cons, nth_error_app2. now replace_nth O. lia.
+  clear XS. intros ??? XS. rewrite DECODE in XS; clear DECODE.
+  change SP with (Z.of_N 13) in XS. change Z_8 with (-Z.of_N 8) in XS.
+  rewrite <-(Z2N.id reg) in XS by lia. 
+  apply exec_str in XS as ?; [|lia..|]. r.
+  apply arm_ls_i_fallthru in XS; [|right;discriminate].
+  left. repeat split. assumption. clear MB; intros MB ?. r.
+
+  apply arm_assemble_all_first in B as [z_ldr [b_tail [B [B_B' DECODE]]]]; subst; rename b_tail into b.
+  eapply afterblock_step. assumption. lia. replace_nth 12%nat. rewrite !nth_error_cons, nth_error_app2. now replace_nth 1%nat. lia.
+  intros ??? XS. rewrite DECODE in XS; clear DECODE.
+  apply arm_ls_i_fallthru in XS; [|left;lia].
+  left. repeat split. assumption. rewrite reset_temps_overwrite_l. clear MB; intros MB ?. r.
+
+  apply arm_assemble_all_first in B as [z_ldr' [b_tail [B [B_B' DECODE]]]]; subst; rename b_tail into b.
+  eapply afterblock_step. assumption. lia. replace_nth 13%nat. rewrite !nth_error_cons, nth_error_app2. now replace_nth 2%nat. lia.
+  intros ??? XS. rewrite DECODE in XS; clear DECODE.
+  eapply exec_ldrpc in XS.
+  right. right. left. eexists. repeat split. apply XS. simpl in RA. shelve. shelve. shelve. shelve. right. mylia. right. mylia. shelve. right. mylia.
+  right. mylia. right. mylia. right. mylia.
+  Unshelve. shelve. all: admit.
   }
   assert (
     forall l cond, arm_assemble_all_cond l cond = Some irm' ->
       (Forall (fun q => forall s c' s' x i a, exec_stmt armc s (arm2il i q) c' s' x  -> x <> Some (Addr a)) l) ->
       (1 <= length l < 64)%nat ->
       In (Z.add i 1) (pol i) ->
-    SafeAfterBlock i2i' pol ai i irm' p s1
+    SafeAfterBlock i2i' pol ai i (length irm') s1
   ) as FT. {
     intros. eapply C. apply H. assumption. assumption.
     destruct arm_assemble_all eqn:e; auto.
     intros. apply afterblock_fallthru'.
       apply arm_assemble_all_eq in e. rewrite <-e, Forall_map in H0. assumption.
       intros. cbv[SafeDestX fst]. right.
-        rewrite N2Z.inj_add, Z2N.id, nat_N_Z in H4 by lia. apply arm_assemble_all_cond_len in H.  apply arm_assemble_all_len in e.
-        remember (_ - _)%nat. assert (n = 0 \/ n = 1)%nat. destruct n. now left. right.  lia. destruct H5. replace (length irm') with (length l0) by lia. now rewrite H5, Z.add_0_r in H4. unfold InBlock in *. split. lia. easy. apply arm_assemble_all_len in e. lia.
-        assumption.
-        intros. cbv[SafeDestX fst SafeDest]. left. right. exists (i+1)%Z. split. unfold i2a', to_a. rewrite <- N.add_assoc, <- Nat2N.inj_add, <-Nat.sub_sub_distr, Nat.sub_diag, Nat.sub_0_r, I2I''. lia. lia. apply arm_assemble_all_cond_len in H. apply arm_assemble_all_len in e. lia. assumption.
+      apply arm_assemble_all_cond_len in H.  apply arm_assemble_all_len in e. unfold InBlock in *. split. lia. easy.
+        apply arm_assemble_all_len in e. lia. assumption.
+        intros. cbv[SafeDestX fst SafeDest]. left. right. exists (i+1)%Z. split. rewrite I2I''. subst i'. apply arm_assemble_all_len in e. apply arm_assemble_all_cond_len in H. lia. assumption.
   }
 
   assert (
@@ -730,7 +1471,7 @@ Proof.
       (forall s c' s' x i a, exec_stmt armc s (arm2il i sanitized_inst) c' s' x  -> x <> Some (Addr a)) ->
       reg <> 15%Z ->
       In (Z.add i 1) (pol i) ->
-    SafeAfterBlock i2i' pol ai i irm' p s1
+    SafeAfterBlock i2i' pol ai i (length irm') s1
   ) as RPNJ. {
     intros. eapply FT. unfold rewrite_pc_no_jump, wo_table in H. destruct_match_in H; try discriminate.
     inversion H. subst. apply e. faft. simpl. lia. assumption.
@@ -742,39 +1483,41 @@ Proof.
       (0 <= reg < 15)%Z ->
       (0 <= reg2 < 15)%Z ->
       In (Z.add i 1) (pol i) ->
-    SafeAfterBlock i2i' pol ai i irm' p s1
+    SafeAfterBlock i2i' pol ai i (length irm') s1
   ) as RPSNJ. {
     intros. eapply FT. unfold rewrite_pc_sp_no_jump, wo_table in H. destruct_match_in H; try discriminate.
     inversion H. subst. apply e. faft. simpl. lia. assumption.
   }
-  assert (goto_abort (i2i' i) ai tc = Some (irm', table, tc') -> SafeAfterBlock i2i' pol ai i irm' p s1) as GA.
+  assert (goto_abort (i2i' i) ai tc = Some (irm', table, tc') -> SafeAfterBlock i2i' pol ai i (length irm') s1) as GA.
   {
     intros. unfold goto_abort in H; destruct_match_in H; try discriminate. inversion H; subst.
-    apply afterblock_cons. assumption. intros. right. right. left. rewrite <-(Z2N.id (i2i' i)), <-(Z2N.id ai) in e by (apply I2I' || lia).
-    eapply GOTOz_correct in e. exists (Z.to_N ai * 4). repeat split. apply e. unfold SafeDestX. simpl. left. left. unfold to_a. lia. now rewrite Z2N.id by apply I2I'. lia. lia. apply H0.
+    eapply afterblock_step. assumption. easy. now replace_nth O. intros. right. right. left. rewrite <-(Z2N.id (i2i' i)), <-(Z2N.id ai) in e by (apply I2I' || lia).
+    eapply GOTOz_correct in e. exists (Z.to_N ai * 4). repeat split. apply e. unfold SafeDestX. simpl. left. left. lia. left. now rewrite Z2N.id by apply I2I'. lia. lia. apply H0.
   }
   assert (
-    irm' = [z] ->
+    irm' = z::nil ->
     In (Z.add i 1) (pol i) ->
     (forall c s c' s' x a, exec_stmt c s (arm2il (Z.to_N (i2i' i) * 4) (arm_decode z)) c' s' x -> x <> Some (Addr a)) ->
-    SafeAfterBlock i2i' pol ai i irm' p s1
+    SafeAfterBlock i2i' pol ai i (length irm') s1
   ) as FTS. {
     intros. subst.
-    apply afterblock_cons. assumption. intros.
-    destruct x eqn:e. destruct e0. now eapply H1 in H. right. right. right. now exists i0. right. left. split. easy. split. easy.
-    unfold SafeDestX, SafeDest. simpl. left. right. exists (Z.add i 1). split. unfold i2a', to_a. rewrite N2Z.inj_mul, N2Z.inj_add, Z2N.id, I2I'', Z.mul_comm. easy.
-    apply I2I'. assumption.
+    eapply afterblock_step. assumption. easy. now replace_nth O. intros.
+    destruct x eqn:e. destruct e0. now eapply H1 in H. right. right. right. now exists i0. right. left. split. easy. split. simpl. lia.
+    unfold SafeDestX, SafeDest. simpl. left. right. exists (Z.add i 1). split. rewrite I2I''. simpl. lia. easy.
   }
 
   unfold rewrite_inst, PC, Z1, Z15 in RI. destruct_match_in RI; try discriminate;
   match type of RI with
   | context[goto_abort] => now apply GA
-  | context[Some ([z], _, _)] => apply FTS; [now inversion RI| rewrite negb_false_iff in e; now apply In_contains in e|faft]
+  | context[Some (z::nil, _, _)] => apply FTS; [now inversion RI| rewrite negb_false_iff in e; now apply In_contains in e|faft]
   | context[rewrite_mov_lr_pc]=>
     unfold rewrite_mov_lr_pc, wo_table in RI; destruct_match_in RI; try discriminate; inversion RI; subst; eapply FT; [apply e4|faft| simpl; lia|rewrite negb_false_iff in e; now apply In_contains in e]
   | context[wo_table]=>
     unfold wo_table in RI; destruct_match_in RI; try discriminate; inversion RI; subst; eapply FT; [apply e6|faft| simpl; lia|rewrite negb_false_iff in e; now apply In_contains in e]
   | context[rewrite_pc_no_jump] => eapply RPNJ; [apply RI|faft|try apply unused_reg_not_pc;easy ..|rewrite negb_false_iff in e;now apply In_contains in e]
   | context[rewrite_pc_sp_no_jump]=> eapply RPSNJ; [apply RI|faft|try apply unused_reg_bound;easy ..|rewrite negb_false_iff in e;now apply In_contains in e]
+  | context[rewrite_bx] => eapply RBX; [apply RI|lia|assumption]
   | _ => clear C GA FT FTS RPNJ RPSNJ
   end.
+Admitted.
+
